ldir-lean/.lake/build/ir/LDIRProofs/proof_ir_wellformedness.c
@@ -45,6 +45,42 @@ LEAN_EXPORT lean_object* lp_LDIRProofs_LDIR_BlockType_code_elim___redArg(lean_ob
 LEAN_EXPORT lean_object* lp_LDIRProofs_LDIR_BlockType_code_elim___redArg___boxed(lean_object*);
 LEAN_EXPORT lean_object* lp_LDIRProofs_LDIR_BlockType_code_elim(lean_object*, uint8_t, lean_object*, lean_object*);
 LEAN_EXPORT lean_object* lp_LDIRProofs_LDIR_BlockType_code_elim___boxed(lean_object*, lean_object*, lean_object*, lean_object*);
+LEAN_EXPORT lean_object* lp_LDIRProofs_LDIR_BlockType_blockQuote_elim___redArg(lean_object*);
+LEAN_EXPORT lean_object* lp_LDIRProofs_LDIR_BlockType_blockQuote_elim___redArg___boxed(lean_object*);
+LEAN_EXPORT lean_object* lp_LDIRProofs_LDIR_BlockType_blockQuote_elim(lean_object*, uint8_t, lean_object*, lean_object*);
+LEAN_EXPORT lean_object* lp_LDIRProofs_LDIR_BlockType_blockQuote_elim___boxed(lean_object*, lean_object*, lean_object*, lean_object*);
+LEAN_EXPORT lean_object* lp_LDIRProofs_LDIR_BlockType_thematicBreak_elim___redArg(lean_object*);
+LEAN_EXPORT lean_object* lp_LDIRProofs_LDIR_BlockType_thematicBreak_elim___redArg___boxed(lean_object*);
+LEAN_EXPORT lean_object* lp_LDIRProofs_LDIR_BlockType_thematicBreak_elim(lean_object*, uint8_t, lean_object*, lean_object*);
+LEAN_EXPORT lean_object* lp_LDIRProofs_LDIR_BlockType_thematicBreak_elim___boxed(lean_object*, lean_object*, lean_object*, lean_object*);
+LEAN_EXPORT lean_object* lp_LDIRProofs_LDIR_BlockType_image_elim___redArg(lean_object*);
+LEAN_EXPORT lean_object* lp_LDIRProofs_LDIR_BlockType_image_elim___redArg___boxed(lean_object*);
+LEAN_EXPORT lean_object* lp_LDIRProofs_LDIR_BlockType_image_elim(lean_object*, uint8_t, lean_object*, lean_object*);
+LEAN_EXPORT lean_object* lp_LDIRProofs_LDIR_BlockType_image_elim___boxed(lean_object*, lean_object*, lean_object*, lean_object*);
+LEAN_EXPORT lean_object* lp_LDIRProofs_LDIR_BlockType_table_elim___redArg(lean_object*);
+LEAN_EXPORT lean_object* lp_LDIRProofs_LDIR_BlockType_table_elim___redArg___boxed(lean_object*);
+LEAN_EXPORT lean_object* lp_LDIRProofs_LDIR_BlockType_table_elim(lean_object*, uint8_t, lean_object*, lean_object*);
+LEAN_EXPORT lean_object* lp_LDIRProofs_LDIR_BlockType_table_elim___boxed(lean_object*, lean_object*, lean_object*, lean_object*);
+LEAN_EXPORT lean_object* lp_LDIRProofs_LDIR_BlockType_tableRow_elim___redArg(lean_object*);
+LEAN_EXPORT lean_object* lp_LDIRProofs_LDIR_BlockType_tableRow_elim___redArg___boxed(lean_object*);
+LEAN_EXPORT lean_object* lp_LDIRProofs_LDIR_BlockType_tableRow_elim(lean_object*, uint8_t, lean_object*, lean_object*);
+LEAN_EXPORT lean_object* lp_LDIRProofs_LDIR_BlockType_tableRow_elim___boxed(lean_object*, lean_object*, lean_object*, lean_object*);
+LEAN_EXPORT lean_object* lp_LDIRProofs_LDIR_BlockType_tableCell_elim___redArg(lean_object*);
+LEAN_EXPORT lean_object* lp_LDIRProofs_LDIR_BlockType_tableCell_elim___redArg___boxed(lean_object*);
+LEAN_EXPORT lean_object* lp_LDIRProofs_LDIR_BlockType_tableCell_elim(lean_object*, uint8_t, lean_object*, lean_object*);
+LEAN_EXPORT lean_object* lp_LDIRProofs_LDIR_BlockType_tableCell_elim___boxed(lean_object*, lean_object*, lean_object*, lean_object*);
+LEAN_EXPORT lean_object* lp_LDIRProofs_LDIR_BlockType_footnote_elim___redArg(lean_object*);
+LEAN_EXPORT lean_object* lp_LDIRProofs_LDIR_BlockType_footnote_elim___redArg___boxed(lean_object*);
+LEAN_EXPORT lean_object* lp_LDIRProofs_LDIR_BlockType_footnote_elim(lean_object*, uint8_t, lean_object*, lean_object*);
+LEAN_EXPORT lean_object* lp_LDIRProofs_LDIR_BlockType_footnote_elim___boxed(lean_object*, lean_object*, lean_object*, lean_object*);
+LEAN_EXPORT lean_object* lp_LDIRProofs_LDIR_BlockType_footnoteBlock_elim___redArg(lean_object*);
+LEAN_EXPORT lean_object* lp_LDIRProofs_LDIR_BlockType_footnoteBlock_elim___redArg___boxed(lean_object*);
+LEAN_EXPORT lean_object* lp_LDIRProofs_LDIR_BlockType_footnoteBlock_elim(lean_object*, uint8_t, lean_object*, lean_object*);
+LEAN_EXPORT lean_object* lp_LDIRProofs_LDIR_BlockType_footnoteBlock_elim___boxed(lean_object*, lean_object*, lean_object*, lean_object*);
+LEAN_EXPORT lean_object* lp_LDIRProofs_LDIR_BlockType_figure_elim___redArg(lean_object*);
+LEAN_EXPORT lean_object* lp_LDIRProofs_LDIR_BlockType_figure_elim___redArg___boxed(lean_object*);
+LEAN_EXPORT lean_object* lp_LDIRProofs_LDIR_BlockType_figure_elim(lean_object*, uint8_t, lean_object*, lean_object*);
+LEAN_EXPORT lean_object* lp_LDIRProofs_LDIR_BlockType_figure_elim___boxed(lean_object*, lean_object*, lean_object*, lean_object*);
 static const lean_string_object lp_LDIRProofs_LDIR_instReprBlockType_repr___closed__0_value = {.m_header = {.m_rc = 0, .m_cs_sz = 0, .m_other = 0, .m_tag = 249}, .m_size = 24, .m_capacity = 24, .m_length = 23, .m_data = "LDIR.BlockType.document"};
 static const lean_object* lp_LDIRProofs_LDIR_instReprBlockType_repr___closed__0 = (const lean_object*)&lp_LDIRProofs_LDIR_instReprBlockType_repr___closed__0_value;
 static const lean_ctor_object lp_LDIRProofs_LDIR_instReprBlockType_repr___closed__1_value = {.m_header = {.m_rc = 0, .m_cs_sz = sizeof(lean_ctor_object) + sizeof(void*)*1 + 0, .m_other = 1, .m_tag = 3}, .m_objs = {((lean_object*)&lp_LDIRProofs_LDIR_instReprBlockType_repr___closed__0_value)}};
@@ -69,11 +105,47 @@ static const lean_string_object lp_LDIRProofs_LDIR_instReprBlockType_repr___clos
 static const lean_object* lp_LDIRProofs_LDIR_instReprBlockType_repr___closed__10 = (const lean_object*)&lp_LDIRProofs_LDIR_instReprBlockType_repr___closed__10_value;
 static const lean_ctor_object lp_LDIRProofs_LDIR_instReprBlockType_repr___closed__11_value = {.m_header = {.m_rc = 0, .m_cs_sz = sizeof(lean_ctor_object) + sizeof(void*)*1 + 0, .m_other = 1, .m_tag = 3}, .m_objs = {((lean_object*)&lp_LDIRProofs_LDIR_instReprBlockType_repr___closed__10_value)}};
 static const lean_object* lp_LDIRProofs_LDIR_instReprBlockType_repr___closed__11 = (const lean_object*)&lp_LDIRProofs_LDIR_instReprBlockType_repr___closed__11_value;
+static const lean_string_object lp_LDIRProofs_LDIR_instReprBlockType_repr___closed__12_value = {.m_header = {.m_rc = 0, .m_cs_sz = 0, .m_other = 0, .m_tag = 249}, .m_size = 26, .m_capacity = 26, .m_length = 25, .m_data = "LDIR.BlockType.blockQuote"};
+static const lean_object* lp_LDIRProofs_LDIR_instReprBlockType_repr___closed__12 = (const lean_object*)&lp_LDIRProofs_LDIR_instReprBlockType_repr___closed__12_value;
+static const lean_ctor_object lp_LDIRProofs_LDIR_instReprBlockType_repr___closed__13_value = {.m_header = {.m_rc = 0, .m_cs_sz = sizeof(lean_ctor_object) + sizeof(void*)*1 + 0, .m_other = 1, .m_tag = 3}, .m_objs = {((lean_object*)&lp_LDIRProofs_LDIR_instReprBlockType_repr___closed__12_value)}};
+static const lean_object* lp_LDIRProofs_LDIR_instReprBlockType_repr___closed__13 = (const lean_object*)&lp_LDIRProofs_LDIR_instReprBlockType_repr___closed__13_value;
+static const lean_string_object lp_LDIRProofs_LDIR_instReprBlockType_repr___closed__14_value = {.m_header = {.m_rc = 0, .m_cs_sz = 0, .m_other = 0, .m_tag = 249}, .m_size = 29, .m_capacity = 29, .m_length = 28, .m_data = "LDIR.BlockType.thematicBreak"};
+static const lean_object* lp_LDIRProofs_LDIR_instReprBlockType_repr___closed__14 = (const lean_object*)&lp_LDIRProofs_LDIR_instReprBlockType_repr___closed__14_value;
+static const lean_ctor_object lp_LDIRProofs_LDIR_instReprBlockType_repr___closed__15_value = {.m_header = {.m_rc = 0, .m_cs_sz = sizeof(lean_ctor_object) + sizeof(void*)*1 + 0, .m_other = 1, .m_tag = 3}, .m_objs = {((lean_object*)&lp_LDIRProofs_LDIR_instReprBlockType_repr___closed__14_value)}};
+static const lean_object* lp_LDIRProofs_LDIR_instReprBlockType_repr___closed__15 = (const lean_object*)&lp_LDIRProofs_LDIR_instReprBlockType_repr___closed__15_value;
+static const lean_string_object lp_LDIRProofs_LDIR_instReprBlockType_repr___closed__16_value = {.m_header = {.m_rc = 0, .m_cs_sz = 0, .m_other = 0, .m_tag = 249}, .m_size = 21, .m_capacity = 21, .m_length = 20, .m_data = "LDIR.BlockType.image"};
+static const lean_object* lp_LDIRProofs_LDIR_instReprBlockType_repr___closed__16 = (const lean_object*)&lp_LDIRProofs_LDIR_instReprBlockType_repr___closed__16_value;
+static const lean_ctor_object lp_LDIRProofs_LDIR_instReprBlockType_repr___closed__17_value = {.m_header = {.m_rc = 0, .m_cs_sz = sizeof(lean_ctor_object) + sizeof(void*)*1 + 0, .m_other = 1, .m_tag = 3}, .m_objs = {((lean_object*)&lp_LDIRProofs_LDIR_instReprBlockType_repr___closed__16_value)}};
+static const lean_object* lp_LDIRProofs_LDIR_instReprBlockType_repr___closed__17 = (const lean_object*)&lp_LDIRProofs_LDIR_instReprBlockType_repr___closed__17_value;
+static const lean_string_object lp_LDIRProofs_LDIR_instReprBlockType_repr___closed__18_value = {.m_header = {.m_rc = 0, .m_cs_sz = 0, .m_other = 0, .m_tag = 249}, .m_size = 21, .m_capacity = 21, .m_length = 20, .m_data = "LDIR.BlockType.table"};
+static const lean_object* lp_LDIRProofs_LDIR_instReprBlockType_repr___closed__18 = (const lean_object*)&lp_LDIRProofs_LDIR_instReprBlockType_repr___closed__18_value;
+static const lean_ctor_object lp_LDIRProofs_LDIR_instReprBlockType_repr___closed__19_value = {.m_header = {.m_rc = 0, .m_cs_sz = sizeof(lean_ctor_object) + sizeof(void*)*1 + 0, .m_other = 1, .m_tag = 3}, .m_objs = {((lean_object*)&lp_LDIRProofs_LDIR_instReprBlockType_repr___closed__18_value)}};
+static const lean_object* lp_LDIRProofs_LDIR_instReprBlockType_repr___closed__19 = (const lean_object*)&lp_LDIRProofs_LDIR_instReprBlockType_repr___closed__19_value;
+static const lean_string_object lp_LDIRProofs_LDIR_instReprBlockType_repr___closed__20_value = {.m_header = {.m_rc = 0, .m_cs_sz = 0, .m_other = 0, .m_tag = 249}, .m_size = 24, .m_capacity = 24, .m_length = 23, .m_data = "LDIR.BlockType.tableRow"};
+static const lean_object* lp_LDIRProofs_LDIR_instReprBlockType_repr___closed__20 = (const lean_object*)&lp_LDIRProofs_LDIR_instReprBlockType_repr___closed__20_value;
+static const lean_ctor_object lp_LDIRProofs_LDIR_instReprBlockType_repr___closed__21_value = {.m_header = {.m_rc = 0, .m_cs_sz = sizeof(lean_ctor_object) + sizeof(void*)*1 + 0, .m_other = 1, .m_tag = 3}, .m_objs = {((lean_object*)&lp_LDIRProofs_LDIR_instReprBlockType_repr___closed__20_value)}};
+static const lean_object* lp_LDIRProofs_LDIR_instReprBlockType_repr___closed__21 = (const lean_object*)&lp_LDIRProofs_LDIR_instReprBlockType_repr___closed__21_value;
+static const lean_string_object lp_LDIRProofs_LDIR_instReprBlockType_repr___closed__22_value = {.m_header = {.m_rc = 0, .m_cs_sz = 0, .m_other = 0, .m_tag = 249}, .m_size = 25, .m_capacity = 25, .m_length = 24, .m_data = "LDIR.BlockType.tableCell"};
+static const lean_object* lp_LDIRProofs_LDIR_instReprBlockType_repr___closed__22 = (const lean_object*)&lp_LDIRProofs_LDIR_instReprBlockType_repr___closed__22_value;
+static const lean_ctor_object lp_LDIRProofs_LDIR_instReprBlockType_repr___closed__23_value = {.m_header = {.m_rc = 0, .m_cs_sz = sizeof(lean_ctor_object) + sizeof(void*)*1 + 0, .m_other = 1, .m_tag = 3}, .m_objs = {((lean_object*)&lp_LDIRProofs_LDIR_instReprBlockType_repr___closed__22_value)}};
+static const lean_object* lp_LDIRProofs_LDIR_instReprBlockType_repr___closed__23 = (const lean_object*)&lp_LDIRProofs_LDIR_instReprBlockType_repr___closed__23_value;
+static const lean_string_object lp_LDIRProofs_LDIR_instReprBlockType_repr___closed__24_value = {.m_header = {.m_rc = 0, .m_cs_sz = 0, .m_other = 0, .m_tag = 249}, .m_size = 24, .m_capacity = 24, .m_length = 23, .m_data = "LDIR.BlockType.footnote"};
+static const lean_object* lp_LDIRProofs_LDIR_instReprBlockType_repr___closed__24 = (const lean_object*)&lp_LDIRProofs_LDIR_instReprBlockType_repr___closed__24_value;
+static const lean_ctor_object lp_LDIRProofs_LDIR_instReprBlockType_repr___closed__25_value = {.m_header = {.m_rc = 0, .m_cs_sz = sizeof(lean_ctor_object) + sizeof(void*)*1 + 0, .m_other = 1, .m_tag = 3}, .m_objs = {((lean_object*)&lp_LDIRProofs_LDIR_instReprBlockType_repr___closed__24_value)}};
+static const lean_object* lp_LDIRProofs_LDIR_instReprBlockType_repr___closed__25 = (const lean_object*)&lp_LDIRProofs_LDIR_instReprBlockType_repr___closed__25_value;
+static const lean_string_object lp_LDIRProofs_LDIR_instReprBlockType_repr___closed__26_value = {.m_header = {.m_rc = 0, .m_cs_sz = 0, .m_other = 0, .m_tag = 249}, .m_size = 29, .m_capacity = 29, .m_length = 28, .m_data = "LDIR.BlockType.footnoteBlock"};
+static const lean_object* lp_LDIRProofs_LDIR_instReprBlockType_repr___closed__26 = (const lean_object*)&lp_LDIRProofs_LDIR_instReprBlockType_repr___closed__26_value;
+static const lean_ctor_object lp_LDIRProofs_LDIR_instReprBlockType_repr___closed__27_value = {.m_header = {.m_rc = 0, .m_cs_sz = sizeof(lean_ctor_object) + sizeof(void*)*1 + 0, .m_other = 1, .m_tag = 3}, .m_objs = {((lean_object*)&lp_LDIRProofs_LDIR_instReprBlockType_repr___closed__26_value)}};
+static const lean_object* lp_LDIRProofs_LDIR_instReprBlockType_repr___closed__27 = (const lean_object*)&lp_LDIRProofs_LDIR_instReprBlockType_repr___closed__27_value;
+static const lean_string_object lp_LDIRProofs_LDIR_instReprBlockType_repr___closed__28_value = {.m_header = {.m_rc = 0, .m_cs_sz = 0, .m_other = 0, .m_tag = 249}, .m_size = 22, .m_capacity = 22, .m_length = 21, .m_data = "LDIR.BlockType.figure"};
+static const lean_object* lp_LDIRProofs_LDIR_instReprBlockType_repr___closed__28 = (const lean_object*)&lp_LDIRProofs_LDIR_instReprBlockType_repr___closed__28_value;
+static const lean_ctor_object lp_LDIRProofs_LDIR_instReprBlockType_repr___closed__29_value = {.m_header = {.m_rc = 0, .m_cs_sz = sizeof(lean_ctor_object) + sizeof(void*)*1 + 0, .m_other = 1, .m_tag = 3}, .m_objs = {((lean_object*)&lp_LDIRProofs_LDIR_instReprBlockType_repr___closed__28_value)}};
+static const lean_object* lp_LDIRProofs_LDIR_instReprBlockType_repr___closed__29 = (const lean_object*)&lp_LDIRProofs_LDIR_instReprBlockType_repr___closed__29_value;
 lean_object* lean_nat_to_int(lean_object*);
-static lean_once_cell_t lp_LDIRProofs_LDIR_instReprBlockType_repr___closed__12_once = LEAN_ONCE_CELL_INITIALIZER;
-static lean_object* lp_LDIRProofs_LDIR_instReprBlockType_repr___closed__12;
-static lean_once_cell_t lp_LDIRProofs_LDIR_instReprBlockType_repr___closed__13_once = LEAN_ONCE_CELL_INITIALIZER;
-static lean_object* lp_LDIRProofs_LDIR_instReprBlockType_repr___closed__13;
+static lean_once_cell_t lp_LDIRProofs_LDIR_instReprBlockType_repr___closed__30_once = LEAN_ONCE_CELL_INITIALIZER;
+static lean_object* lp_LDIRProofs_LDIR_instReprBlockType_repr___closed__30;
+static lean_once_cell_t lp_LDIRProofs_LDIR_instReprBlockType_repr___closed__31_once = LEAN_ONCE_CELL_INITIALIZER;
+static lean_object* lp_LDIRProofs_LDIR_instReprBlockType_repr___closed__31;
 lean_object* l_Repr_addAppParen(lean_object*, lean_object*);
 uint8_t lean_nat_dec_le(lean_object*, lean_object*);
 LEAN_EXPORT lean_object* lp_LDIRProofs_LDIR_instReprBlockType_repr(uint8_t, lean_object*);
@@ -214,6 +286,83 @@ LEAN_EXPORT lean_object* lp_LDIRProofs_LDIR_instBEqSIRInstruction_beq___boxed(le
 static const lean_closure_object lp_LDIRProofs_LDIR_instBEqSIRInstruction___closed__0_value = {.m_header = {.m_rc = 0, .m_cs_sz = sizeof(lean_closure_object) + sizeof(void*)*0, .m_other = 0, .m_tag = 245}, .m_fun = (void*)lp_LDIRProofs_LDIR_instBEqSIRInstruction_beq___boxed, .m_arity = 2, .m_num_fixed = 0, .m_objs = {} };
 static const lean_object* lp_LDIRProofs_LDIR_instBEqSIRInstruction___closed__0 = (const lean_object*)&lp_LDIRProofs_LDIR_instBEqSIRInstruction___closed__0_value;
 LEAN_EXPORT const lean_object* lp_LDIRProofs_LDIR_instBEqSIRInstruction = (const lean_object*)&lp_LDIRProofs_LDIR_instBEqSIRInstruction___closed__0_value;
+static const lean_string_object lp_LDIRProofs_LDIR_instReprPayloadTable_repr___redArg___closed__0_value = {.m_header = {.m_rc = 0, .m_cs_sz = 0, .m_other = 0, .m_tag = 249}, .m_size = 5, .m_capacity = 5, .m_length = 4, .m_data = "data"};
+static const lean_object* lp_LDIRProofs_LDIR_instReprPayloadTable_repr___redArg___closed__0 = (const lean_object*)&lp_LDIRProofs_LDIR_instReprPayloadTable_repr___redArg___closed__0_value;
+static const lean_ctor_object lp_LDIRProofs_LDIR_instReprPayloadTable_repr___redArg___closed__1_value = {.m_header = {.m_rc = 0, .m_cs_sz = sizeof(lean_ctor_object) + sizeof(void*)*1 + 0, .m_other = 1, .m_tag = 3}, .m_objs = {((lean_object*)&lp_LDIRProofs_LDIR_instReprPayloadTable_repr___redArg___closed__0_value)}};
+static const lean_object* lp_LDIRProofs_LDIR_instReprPayloadTable_repr___redArg___closed__1 = (const lean_object*)&lp_LDIRProofs_LDIR_instReprPayloadTable_repr___redArg___closed__1_value;
+static const lean_ctor_object lp_LDIRProofs_LDIR_instReprPayloadTable_repr___redArg___closed__2_value = {.m_header = {.m_rc = 0, .m_cs_sz = sizeof(lean_ctor_object) + sizeof(void*)*2 + 0, .m_other = 2, .m_tag = 5}, .m_objs = {((lean_object*)(((size_t)(0) << 1) | 1)),((lean_object*)&lp_LDIRProofs_LDIR_instReprPayloadTable_repr___redArg___closed__1_value)}};
+static const lean_object* lp_LDIRProofs_LDIR_instReprPayloadTable_repr___redArg___closed__2 = (const lean_object*)&lp_LDIRProofs_LDIR_instReprPayloadTable_repr___redArg___closed__2_value;
+static const lean_ctor_object lp_LDIRProofs_LDIR_instReprPayloadTable_repr___redArg___closed__3_value = {.m_header = {.m_rc = 0, .m_cs_sz = sizeof(lean_ctor_object) + sizeof(void*)*2 + 0, .m_other = 2, .m_tag = 5}, .m_objs = {((lean_object*)&lp_LDIRProofs_LDIR_instReprPayloadTable_repr___redArg___closed__2_value),((lean_object*)&lp_LDIRProofs_LDIR_instReprSIRInstruction_repr___redArg___closed__5_value)}};
+static const lean_object* lp_LDIRProofs_LDIR_instReprPayloadTable_repr___redArg___closed__3 = (const lean_object*)&lp_LDIRProofs_LDIR_instReprPayloadTable_repr___redArg___closed__3_value;
+static lean_once_cell_t lp_LDIRProofs_LDIR_instReprPayloadTable_repr___redArg___closed__4_once = LEAN_ONCE_CELL_INITIALIZER;
+static lean_object* lp_LDIRProofs_LDIR_instReprPayloadTable_repr___redArg___closed__4;
+lean_object* l_String_quote(lean_object*);
+LEAN_EXPORT lean_object* lp_LDIRProofs_LDIR_instReprPayloadTable_repr___redArg(lean_object*);
+LEAN_EXPORT lean_object* lp_LDIRProofs_LDIR_instReprPayloadTable_repr(lean_object*, lean_object*);
+LEAN_EXPORT lean_object* lp_LDIRProofs_LDIR_instReprPayloadTable_repr___boxed(lean_object*, lean_object*);
+static const lean_closure_object lp_LDIRProofs_LDIR_instReprPayloadTable___closed__0_value = {.m_header = {.m_rc = 0, .m_cs_sz = sizeof(lean_closure_object) + sizeof(void*)*0, .m_other = 0, .m_tag = 245}, .m_fun = (void*)lp_LDIRProofs_LDIR_instReprPayloadTable_repr___boxed, .m_arity = 2, .m_num_fixed = 0, .m_objs = {} };
+static const lean_object* lp_LDIRProofs_LDIR_instReprPayloadTable___closed__0 = (const lean_object*)&lp_LDIRProofs_LDIR_instReprPayloadTable___closed__0_value;
+LEAN_EXPORT const lean_object* lp_LDIRProofs_LDIR_instReprPayloadTable = (const lean_object*)&lp_LDIRProofs_LDIR_instReprPayloadTable___closed__0_value;
+uint8_t lean_string_dec_eq(lean_object*, lean_object*);
+LEAN_EXPORT uint8_t lp_LDIRProofs_LDIR_instBEqPayloadTable_beq(lean_object*, lean_object*);
+LEAN_EXPORT lean_object* lp_LDIRProofs_LDIR_instBEqPayloadTable_beq___boxed(lean_object*, lean_object*);
+static const lean_closure_object lp_LDIRProofs_LDIR_instBEqPayloadTable___closed__0_value = {.m_header = {.m_rc = 0, .m_cs_sz = sizeof(lean_closure_object) + sizeof(void*)*0, .m_other = 0, .m_tag = 245}, .m_fun = (void*)lp_LDIRProofs_LDIR_instBEqPayloadTable_beq___boxed, .m_arity = 2, .m_num_fixed = 0, .m_objs = {} };
+static const lean_object* lp_LDIRProofs_LDIR_instBEqPayloadTable___closed__0 = (const lean_object*)&lp_LDIRProofs_LDIR_instBEqPayloadTable___closed__0_value;
+LEAN_EXPORT const lean_object* lp_LDIRProofs_LDIR_instBEqPayloadTable = (const lean_object*)&lp_LDIRProofs_LDIR_instBEqPayloadTable___closed__0_value;
+LEAN_EXPORT lean_object* lp_LDIRProofs_List_foldl___at___00List_foldl___at___00Std_Format_joinSep___at___00List_repr___at___00LDIR_instReprSIRDocumentWithPayload_repr_spec__0_spec__0_spec__1_spec__2(lean_object*, lean_object*, lean_object*);
+LEAN_EXPORT lean_object* lp_LDIRProofs_List_foldl___at___00Std_Format_joinSep___at___00List_repr___at___00LDIR_instReprSIRDocumentWithPayload_repr_spec__0_spec__0_spec__1(lean_object*, lean_object*, lean_object*);
+LEAN_EXPORT lean_object* lp_LDIRProofs_Std_Format_joinSep___at___00List_repr___at___00LDIR_instReprSIRDocumentWithPayload_repr_spec__0_spec__0(lean_object*, lean_object*);
+static const lean_string_object lp_LDIRProofs_List_repr___at___00LDIR_instReprSIRDocumentWithPayload_repr_spec__0___redArg___closed__0_value = {.m_header = {.m_rc = 0, .m_cs_sz = 0, .m_other = 0, .m_tag = 249}, .m_size = 3, .m_capacity = 3, .m_length = 2, .m_data = "[]"};
+static const lean_object* lp_LDIRProofs_List_repr___at___00LDIR_instReprSIRDocumentWithPayload_repr_spec__0___redArg___closed__0 = (const lean_object*)&lp_LDIRProofs_List_repr___at___00LDIR_instReprSIRDocumentWithPayload_repr_spec__0___redArg___closed__0_value;
+static const lean_ctor_object lp_LDIRProofs_List_repr___at___00LDIR_instReprSIRDocumentWithPayload_repr_spec__0___redArg___closed__1_value = {.m_header = {.m_rc = 0, .m_cs_sz = sizeof(lean_ctor_object) + sizeof(void*)*1 + 0, .m_other = 1, .m_tag = 3}, .m_objs = {((lean_object*)&lp_LDIRProofs_List_repr___at___00LDIR_instReprSIRDocumentWithPayload_repr_spec__0___redArg___closed__0_value)}};
+static const lean_object* lp_LDIRProofs_List_repr___at___00LDIR_instReprSIRDocumentWithPayload_repr_spec__0___redArg___closed__1 = (const lean_object*)&lp_LDIRProofs_List_repr___at___00LDIR_instReprSIRDocumentWithPayload_repr_spec__0___redArg___closed__1_value;
+static const lean_string_object lp_LDIRProofs_List_repr___at___00LDIR_instReprSIRDocumentWithPayload_repr_spec__0___redArg___closed__2_value = {.m_header = {.m_rc = 0, .m_cs_sz = 0, .m_other = 0, .m_tag = 249}, .m_size = 2, .m_capacity = 2, .m_length = 1, .m_data = "["};
+static const lean_object* lp_LDIRProofs_List_repr___at___00LDIR_instReprSIRDocumentWithPayload_repr_spec__0___redArg___closed__2 = (const lean_object*)&lp_LDIRProofs_List_repr___at___00LDIR_instReprSIRDocumentWithPayload_repr_spec__0___redArg___closed__2_value;
+static const lean_ctor_object lp_LDIRProofs_List_repr___at___00LDIR_instReprSIRDocumentWithPayload_repr_spec__0___redArg___closed__3_value = {.m_header = {.m_rc = 0, .m_cs_sz = sizeof(lean_ctor_object) + sizeof(void*)*2 + 0, .m_other = 2, .m_tag = 5}, .m_objs = {((lean_object*)&lp_LDIRProofs_LDIR_instReprSIRInstruction_repr___redArg___closed__9_value),((lean_object*)(((size_t)(1) << 1) | 1))}};
+static const lean_object* lp_LDIRProofs_List_repr___at___00LDIR_instReprSIRDocumentWithPayload_repr_spec__0___redArg___closed__3 = (const lean_object*)&lp_LDIRProofs_List_repr___at___00LDIR_instReprSIRDocumentWithPayload_repr_spec__0___redArg___closed__3_value;
+static const lean_string_object lp_LDIRProofs_List_repr___at___00LDIR_instReprSIRDocumentWithPayload_repr_spec__0___redArg___closed__4_value = {.m_header = {.m_rc = 0, .m_cs_sz = 0, .m_other = 0, .m_tag = 249}, .m_size = 2, .m_capacity = 2, .m_length = 1, .m_data = "]"};
+static const lean_object* lp_LDIRProofs_List_repr___at___00LDIR_instReprSIRDocumentWithPayload_repr_spec__0___redArg___closed__4 = (const lean_object*)&lp_LDIRProofs_List_repr___at___00LDIR_instReprSIRDocumentWithPayload_repr_spec__0___redArg___closed__4_value;
+static lean_once_cell_t lp_LDIRProofs_List_repr___at___00LDIR_instReprSIRDocumentWithPayload_repr_spec__0___redArg___closed__5_once = LEAN_ONCE_CELL_INITIALIZER;
+static lean_object* lp_LDIRProofs_List_repr___at___00LDIR_instReprSIRDocumentWithPayload_repr_spec__0___redArg___closed__5;
+static lean_once_cell_t lp_LDIRProofs_List_repr___at___00LDIR_instReprSIRDocumentWithPayload_repr_spec__0___redArg___closed__6_once = LEAN_ONCE_CELL_INITIALIZER;
+static lean_object* lp_LDIRProofs_List_repr___at___00LDIR_instReprSIRDocumentWithPayload_repr_spec__0___redArg___closed__6;
+static const lean_ctor_object lp_LDIRProofs_List_repr___at___00LDIR_instReprSIRDocumentWithPayload_repr_spec__0___redArg___closed__7_value = {.m_header = {.m_rc = 0, .m_cs_sz = sizeof(lean_ctor_object) + sizeof(void*)*1 + 0, .m_other = 1, .m_tag = 3}, .m_objs = {((lean_object*)&lp_LDIRProofs_List_repr___at___00LDIR_instReprSIRDocumentWithPayload_repr_spec__0___redArg___closed__2_value)}};
+static const lean_object* lp_LDIRProofs_List_repr___at___00LDIR_instReprSIRDocumentWithPayload_repr_spec__0___redArg___closed__7 = (const lean_object*)&lp_LDIRProofs_List_repr___at___00LDIR_instReprSIRDocumentWithPayload_repr_spec__0___redArg___closed__7_value;
+static const lean_ctor_object lp_LDIRProofs_List_repr___at___00LDIR_instReprSIRDocumentWithPayload_repr_spec__0___redArg___closed__8_value = {.m_header = {.m_rc = 0, .m_cs_sz = sizeof(lean_ctor_object) + sizeof(void*)*1 + 0, .m_other = 1, .m_tag = 3}, .m_objs = {((lean_object*)&lp_LDIRProofs_List_repr___at___00LDIR_instReprSIRDocumentWithPayload_repr_spec__0___redArg___closed__4_value)}};
+static const lean_object* lp_LDIRProofs_List_repr___at___00LDIR_instReprSIRDocumentWithPayload_repr_spec__0___redArg___closed__8 = (const lean_object*)&lp_LDIRProofs_List_repr___at___00LDIR_instReprSIRDocumentWithPayload_repr_spec__0___redArg___closed__8_value;
+LEAN_EXPORT lean_object* lp_LDIRProofs_List_repr___at___00LDIR_instReprSIRDocumentWithPayload_repr_spec__0___redArg(lean_object*);
+static const lean_string_object lp_LDIRProofs_LDIR_instReprSIRDocumentWithPayload_repr___redArg___closed__0_value = {.m_header = {.m_rc = 0, .m_cs_sz = 0, .m_other = 0, .m_tag = 249}, .m_size = 13, .m_capacity = 13, .m_length = 12, .m_data = "instructions"};
+static const lean_object* lp_LDIRProofs_LDIR_instReprSIRDocumentWithPayload_repr___redArg___closed__0 = (const lean_object*)&lp_LDIRProofs_LDIR_instReprSIRDocumentWithPayload_repr___redArg___closed__0_value;
+static const lean_ctor_object lp_LDIRProofs_LDIR_instReprSIRDocumentWithPayload_repr___redArg___closed__1_value = {.m_header = {.m_rc = 0, .m_cs_sz = sizeof(lean_ctor_object) + sizeof(void*)*1 + 0, .m_other = 1, .m_tag = 3}, .m_objs = {((lean_object*)&lp_LDIRProofs_LDIR_instReprSIRDocumentWithPayload_repr___redArg___closed__0_value)}};
+static const lean_object* lp_LDIRProofs_LDIR_instReprSIRDocumentWithPayload_repr___redArg___closed__1 = (const lean_object*)&lp_LDIRProofs_LDIR_instReprSIRDocumentWithPayload_repr___redArg___closed__1_value;
+static const lean_ctor_object lp_LDIRProofs_LDIR_instReprSIRDocumentWithPayload_repr___redArg___closed__2_value = {.m_header = {.m_rc = 0, .m_cs_sz = sizeof(lean_ctor_object) + sizeof(void*)*2 + 0, .m_other = 2, .m_tag = 5}, .m_objs = {((lean_object*)(((size_t)(0) << 1) | 1)),((lean_object*)&lp_LDIRProofs_LDIR_instReprSIRDocumentWithPayload_repr___redArg___closed__1_value)}};
+static const lean_object* lp_LDIRProofs_LDIR_instReprSIRDocumentWithPayload_repr___redArg___closed__2 = (const lean_object*)&lp_LDIRProofs_LDIR_instReprSIRDocumentWithPayload_repr___redArg___closed__2_value;
+static const lean_ctor_object lp_LDIRProofs_LDIR_instReprSIRDocumentWithPayload_repr___redArg___closed__3_value = {.m_header = {.m_rc = 0, .m_cs_sz = sizeof(lean_ctor_object) + sizeof(void*)*2 + 0, .m_other = 2, .m_tag = 5}, .m_objs = {((lean_object*)&lp_LDIRProofs_LDIR_instReprSIRDocumentWithPayload_repr___redArg___closed__2_value),((lean_object*)&lp_LDIRProofs_LDIR_instReprSIRInstruction_repr___redArg___closed__5_value)}};
+static const lean_object* lp_LDIRProofs_LDIR_instReprSIRDocumentWithPayload_repr___redArg___closed__3 = (const lean_object*)&lp_LDIRProofs_LDIR_instReprSIRDocumentWithPayload_repr___redArg___closed__3_value;
+static lean_once_cell_t lp_LDIRProofs_LDIR_instReprSIRDocumentWithPayload_repr___redArg___closed__4_once = LEAN_ONCE_CELL_INITIALIZER;
+static lean_object* lp_LDIRProofs_LDIR_instReprSIRDocumentWithPayload_repr___redArg___closed__4;
+static const lean_string_object lp_LDIRProofs_LDIR_instReprSIRDocumentWithPayload_repr___redArg___closed__5_value = {.m_header = {.m_rc = 0, .m_cs_sz = 0, .m_other = 0, .m_tag = 249}, .m_size = 8, .m_capacity = 8, .m_length = 7, .m_data = "payload"};
+static const lean_object* lp_LDIRProofs_LDIR_instReprSIRDocumentWithPayload_repr___redArg___closed__5 = (const lean_object*)&lp_LDIRProofs_LDIR_instReprSIRDocumentWithPayload_repr___redArg___closed__5_value;
+static const lean_ctor_object lp_LDIRProofs_LDIR_instReprSIRDocumentWithPayload_repr___redArg___closed__6_value = {.m_header = {.m_rc = 0, .m_cs_sz = sizeof(lean_ctor_object) + sizeof(void*)*1 + 0, .m_other = 1, .m_tag = 3}, .m_objs = {((lean_object*)&lp_LDIRProofs_LDIR_instReprSIRDocumentWithPayload_repr___redArg___closed__5_value)}};
+static const lean_object* lp_LDIRProofs_LDIR_instReprSIRDocumentWithPayload_repr___redArg___closed__6 = (const lean_object*)&lp_LDIRProofs_LDIR_instReprSIRDocumentWithPayload_repr___redArg___closed__6_value;
+static lean_once_cell_t lp_LDIRProofs_LDIR_instReprSIRDocumentWithPayload_repr___redArg___closed__7_once = LEAN_ONCE_CELL_INITIALIZER;
+static lean_object* lp_LDIRProofs_LDIR_instReprSIRDocumentWithPayload_repr___redArg___closed__7;
+LEAN_EXPORT lean_object* lp_LDIRProofs_LDIR_instReprSIRDocumentWithPayload_repr___redArg(lean_object*);
+LEAN_EXPORT lean_object* lp_LDIRProofs_LDIR_instReprSIRDocumentWithPayload_repr(lean_object*, lean_object*);
+LEAN_EXPORT lean_object* lp_LDIRProofs_LDIR_instReprSIRDocumentWithPayload_repr___boxed(lean_object*, lean_object*);
+LEAN_EXPORT lean_object* lp_LDIRProofs_List_repr___at___00LDIR_instReprSIRDocumentWithPayload_repr_spec__0(lean_object*, lean_object*);
+LEAN_EXPORT lean_object* lp_LDIRProofs_List_repr___at___00LDIR_instReprSIRDocumentWithPayload_repr_spec__0___boxed(lean_object*, lean_object*);
+static const lean_closure_object lp_LDIRProofs_LDIR_instReprSIRDocumentWithPayload___closed__0_value = {.m_header = {.m_rc = 0, .m_cs_sz = sizeof(lean_closure_object) + sizeof(void*)*0, .m_other = 0, .m_tag = 245}, .m_fun = (void*)lp_LDIRProofs_LDIR_instReprSIRDocumentWithPayload_repr___boxed, .m_arity = 2, .m_num_fixed = 0, .m_objs = {} };
+static const lean_object* lp_LDIRProofs_LDIR_instReprSIRDocumentWithPayload___closed__0 = (const lean_object*)&lp_LDIRProofs_LDIR_instReprSIRDocumentWithPayload___closed__0_value;
+LEAN_EXPORT const lean_object* lp_LDIRProofs_LDIR_instReprSIRDocumentWithPayload = (const lean_object*)&lp_LDIRProofs_LDIR_instReprSIRDocumentWithPayload___closed__0_value;
+LEAN_EXPORT uint8_t lp_LDIRProofs_List_beq___at___00LDIR_instBEqSIRDocumentWithPayload_beq_spec__0(lean_object*, lean_object*);
+LEAN_EXPORT lean_object* lp_LDIRProofs_List_beq___at___00LDIR_instBEqSIRDocumentWithPayload_beq_spec__0___boxed(lean_object*, lean_object*);
+LEAN_EXPORT uint8_t lp_LDIRProofs_LDIR_instBEqSIRDocumentWithPayload_beq(lean_object*, lean_object*);
+LEAN_EXPORT lean_object* lp_LDIRProofs_LDIR_instBEqSIRDocumentWithPayload_beq___boxed(lean_object*, lean_object*);
+static const lean_closure_object lp_LDIRProofs_LDIR_instBEqSIRDocumentWithPayload___closed__0_value = {.m_header = {.m_rc = 0, .m_cs_sz = sizeof(lean_closure_object) + sizeof(void*)*0, .m_other = 0, .m_tag = 245}, .m_fun = (void*)lp_LDIRProofs_LDIR_instBEqSIRDocumentWithPayload_beq___boxed, .m_arity = 2, .m_num_fixed = 0, .m_objs = {} };
+static const lean_object* lp_LDIRProofs_LDIR_instBEqSIRDocumentWithPayload___closed__0 = (const lean_object*)&lp_LDIRProofs_LDIR_instBEqSIRDocumentWithPayload___closed__0_value;
+LEAN_EXPORT const lean_object* lp_LDIRProofs_LDIR_instBEqSIRDocumentWithPayload = (const lean_object*)&lp_LDIRProofs_LDIR_instBEqSIRDocumentWithPayload___closed__0_value;
+LEAN_EXPORT lean_object* lp_LDIRProofs_LDIR_GIR__COMMAND__ARGS;
 LEAN_EXPORT lean_object* lp_LDIRProofs_LDIR_GIROpcode_ctorIdx(uint8_t);
 LEAN_EXPORT lean_object* lp_LDIRProofs_LDIR_GIROpcode_ctorIdx___boxed(lean_object*);
 LEAN_EXPORT lean_object* lp_LDIRProofs_LDIR_GIROpcode_toCtorIdx(uint8_t);
@@ -292,32 +441,26 @@ LEAN_EXPORT uint8_t lp_LDIRProofs_LDIR_GIROpcode_ofNat(lean_object*);
 LEAN_EXPORT lean_object* lp_LDIRProofs_LDIR_GIROpcode_ofNat___boxed(lean_object*);
 LEAN_EXPORT uint8_t lp_LDIRProofs_LDIR_instDecidableEqGIROpcode(uint8_t, uint8_t);
 LEAN_EXPORT lean_object* lp_LDIRProofs_LDIR_instDecidableEqGIROpcode___boxed(lean_object*, lean_object*);
-static const lean_string_object lp_LDIRProofs_LDIR_instReprGIRCommand_repr___redArg___closed__0_value = {.m_header = {.m_rc = 0, .m_cs_sz = 0, .m_other = 0, .m_tag = 249}, .m_size = 7, .m_capacity = 7, .m_length = 6, .m_data = "argInt"};
-static const lean_object* lp_LDIRProofs_LDIR_instReprGIRCommand_repr___redArg___closed__0 = (const lean_object*)&lp_LDIRProofs_LDIR_instReprGIRCommand_repr___redArg___closed__0_value;
-static const lean_ctor_object lp_LDIRProofs_LDIR_instReprGIRCommand_repr___redArg___closed__1_value = {.m_header = {.m_rc = 0, .m_cs_sz = sizeof(lean_ctor_object) + sizeof(void*)*1 + 0, .m_other = 1, .m_tag = 3}, .m_objs = {((lean_object*)&lp_LDIRProofs_LDIR_instReprGIRCommand_repr___redArg___closed__0_value)}};
-static const lean_object* lp_LDIRProofs_LDIR_instReprGIRCommand_repr___redArg___closed__1 = (const lean_object*)&lp_LDIRProofs_LDIR_instReprGIRCommand_repr___redArg___closed__1_value;
-static const lean_string_object lp_LDIRProofs_LDIR_instReprGIRCommand_repr___redArg___closed__2_value = {.m_header = {.m_rc = 0, .m_cs_sz = 0, .m_other = 0, .m_tag = 249}, .m_size = 7, .m_capacity = 7, .m_length = 6, .m_data = "argStr"};
-static const lean_object* lp_LDIRProofs_LDIR_instReprGIRCommand_repr___redArg___closed__2 = (const lean_object*)&lp_LDIRProofs_LDIR_instReprGIRCommand_repr___redArg___closed__2_value;
-static const lean_ctor_object lp_LDIRProofs_LDIR_instReprGIRCommand_repr___redArg___closed__3_value = {.m_header = {.m_rc = 0, .m_cs_sz = sizeof(lean_ctor_object) + sizeof(void*)*1 + 0, .m_other = 1, .m_tag = 3}, .m_objs = {((lean_object*)&lp_LDIRProofs_LDIR_instReprGIRCommand_repr___redArg___closed__2_value)}};
-static const lean_object* lp_LDIRProofs_LDIR_instReprGIRCommand_repr___redArg___closed__3 = (const lean_object*)&lp_LDIRProofs_LDIR_instReprGIRCommand_repr___redArg___closed__3_value;
-static lean_once_cell_t lp_LDIRProofs_LDIR_instReprGIRCommand_repr___redArg___closed__4_once = LEAN_ONCE_CELL_INITIALIZER;
-static lean_object* lp_LDIRProofs_LDIR_instReprGIRCommand_repr___redArg___closed__4;
-lean_object* l_String_quote(lean_object*);
-uint8_t lean_int_dec_lt(lean_object*, lean_object*);
-lean_object* l_Int_repr(lean_object*);
-LEAN_EXPORT lean_object* lp_LDIRProofs_LDIR_instReprGIRCommand_repr___redArg(lean_object*);
-LEAN_EXPORT lean_object* lp_LDIRProofs_LDIR_instReprGIRCommand_repr(lean_object*, lean_object*);
-LEAN_EXPORT lean_object* lp_LDIRProofs_LDIR_instReprGIRCommand_repr___boxed(lean_object*, lean_object*);
-static const lean_closure_object lp_LDIRProofs_LDIR_instReprGIRCommand___closed__0_value = {.m_header = {.m_rc = 0, .m_cs_sz = sizeof(lean_closure_object) + sizeof(void*)*0, .m_other = 0, .m_tag = 245}, .m_fun = (void*)lp_LDIRProofs_LDIR_instReprGIRCommand_repr___boxed, .m_arity = 2, .m_num_fixed = 0, .m_objs = {} };
-static const lean_object* lp_LDIRProofs_LDIR_instReprGIRCommand___closed__0 = (const lean_object*)&lp_LDIRProofs_LDIR_instReprGIRCommand___closed__0_value;
-LEAN_EXPORT const lean_object* lp_LDIRProofs_LDIR_instReprGIRCommand = (const lean_object*)&lp_LDIRProofs_LDIR_instReprGIRCommand___closed__0_value;
+static lean_once_cell_t lp_LDIRProofs_LDIR_GIRCommand_zeroed___lam__0___closed__0_once = LEAN_ONCE_CELL_INITIALIZER;
+static lean_object* lp_LDIRProofs_LDIR_GIRCommand_zeroed___lam__0___closed__0;
+LEAN_EXPORT lean_object* lp_LDIRProofs_LDIR_GIRCommand_zeroed___lam__0(lean_object*);
+LEAN_EXPORT lean_object* lp_LDIRProofs_LDIR_GIRCommand_zeroed___lam__0___boxed(lean_object*);
+static const lean_closure_object lp_LDIRProofs_LDIR_GIRCommand_zeroed___closed__0_value = {.m_header = {.m_rc = 0, .m_cs_sz = sizeof(lean_closure_object) + sizeof(void*)*0, .m_other = 0, .m_tag = 245}, .m_fun = (void*)lp_LDIRProofs_LDIR_GIRCommand_zeroed___lam__0___boxed, .m_arity = 1, .m_num_fixed = 0, .m_objs = {} };
+static const lean_object* lp_LDIRProofs_LDIR_GIRCommand_zeroed___closed__0 = (const lean_object*)&lp_LDIRProofs_LDIR_GIRCommand_zeroed___closed__0_value;
+LEAN_EXPORT lean_object* lp_LDIRProofs_LDIR_GIRCommand_zeroed(uint8_t);
+LEAN_EXPORT lean_object* lp_LDIRProofs_LDIR_GIRCommand_zeroed___boxed(lean_object*);
 uint8_t lean_int_dec_eq(lean_object*, lean_object*);
-uint8_t lean_string_dec_eq(lean_object*, lean_object*);
-LEAN_EXPORT uint8_t lp_LDIRProofs_LDIR_instBEqGIRCommand_beq(lean_object*, lean_object*);
-LEAN_EXPORT lean_object* lp_LDIRProofs_LDIR_instBEqGIRCommand_beq___boxed(lean_object*, lean_object*);
-static const lean_closure_object lp_LDIRProofs_LDIR_instBEqGIRCommand___closed__0_value = {.m_header = {.m_rc = 0, .m_cs_sz = sizeof(lean_closure_object) + sizeof(void*)*0, .m_other = 0, .m_tag = 245}, .m_fun = (void*)lp_LDIRProofs_LDIR_instBEqGIRCommand_beq___boxed, .m_arity = 2, .m_num_fixed = 0, .m_objs = {} };
+LEAN_EXPORT uint8_t lp_LDIRProofs_LDIR_instBEqGIRCommand___lam__0(lean_object*, lean_object*, lean_object*);
+LEAN_EXPORT lean_object* lp_LDIRProofs_LDIR_instBEqGIRCommand___lam__0___boxed(lean_object*, lean_object*, lean_object*);
+uint8_t l_Nat_decidableForallFin___redArg(lean_object*, lean_object*);
+LEAN_EXPORT uint8_t lp_LDIRProofs_LDIR_instBEqGIRCommand___lam__1(lean_object*, lean_object*);
+LEAN_EXPORT lean_object* lp_LDIRProofs_LDIR_instBEqGIRCommand___lam__1___boxed(lean_object*, lean_object*);
+static const lean_closure_object lp_LDIRProofs_LDIR_instBEqGIRCommand___closed__0_value = {.m_header = {.m_rc = 0, .m_cs_sz = sizeof(lean_closure_object) + sizeof(void*)*0, .m_other = 0, .m_tag = 245}, .m_fun = (void*)lp_LDIRProofs_LDIR_instBEqGIRCommand___lam__1___boxed, .m_arity = 2, .m_num_fixed = 0, .m_objs = {} };
 static const lean_object* lp_LDIRProofs_LDIR_instBEqGIRCommand___closed__0 = (const lean_object*)&lp_LDIRProofs_LDIR_instBEqGIRCommand___closed__0_value;
 LEAN_EXPORT const lean_object* lp_LDIRProofs_LDIR_instBEqGIRCommand = (const lean_object*)&lp_LDIRProofs_LDIR_instBEqGIRCommand___closed__0_value;
+static lean_once_cell_t lp_LDIRProofs_LDIR_instInhabitedGIRCommand___closed__0_once = LEAN_ONCE_CELL_INITIALIZER;
+static lean_object* lp_LDIRProofs_LDIR_instInhabitedGIRCommand___closed__0;
+LEAN_EXPORT lean_object* lp_LDIRProofs_LDIR_instInhabitedGIRCommand;
 lean_object* l_List_reverse___redArg(lean_object*);
 LEAN_EXPORT lean_object* lp_LDIRProofs_List_mapTR_loop___at___00LDIR_entityUnique_spec__0(lean_object*, lean_object*);
 lean_object* l_instDecidableEqNat___boxed(lean_object*, lean_object*);
@@ -339,12 +482,28 @@ LEAN_EXPORT lean_object* lp_LDIRProofs_List_filterTR_loop___at___00LDIR_hasSingl
 lean_object* l_List_lengthTR___redArg(lean_object*);
 LEAN_EXPORT uint8_t lp_LDIRProofs_LDIR_hasSingleRoot(lean_object*);
 LEAN_EXPORT lean_object* lp_LDIRProofs_LDIR_hasSingleRoot___boxed(lean_object*);
+LEAN_EXPORT uint8_t lp_LDIRProofs_LDIR_isAcyclicAux___lam__0(lean_object*, lean_object*);
+LEAN_EXPORT lean_object* lp_LDIRProofs_LDIR_isAcyclicAux___lam__0___boxed(lean_object*, lean_object*);
+lean_object* l_List_find_x3f___redArg(lean_object*, lean_object*);
+lean_object* lean_nat_sub(lean_object*, lean_object*);
+LEAN_EXPORT uint8_t lp_LDIRProofs_LDIR_isAcyclicAux(lean_object*, lean_object*, lean_object*);
+LEAN_EXPORT lean_object* lp_LDIRProofs_LDIR_isAcyclicAux___boxed(lean_object*, lean_object*, lean_object*);
+LEAN_EXPORT uint8_t lp_LDIRProofs_LDIR_isAcyclic___lam__0(lean_object*, lean_object*);
+LEAN_EXPORT lean_object* lp_LDIRProofs_LDIR_isAcyclic___lam__0___boxed(lean_object*, lean_object*);
+LEAN_EXPORT uint8_t lp_LDIRProofs_LDIR_isAcyclic(lean_object*);
+LEAN_EXPORT lean_object* lp_LDIRProofs_LDIR_isAcyclic___boxed(lean_object*);
+lean_object* lean_string_length(lean_object*);
+uint8_t lean_nat_dec_lt(lean_object*, lean_object*);
+LEAN_EXPORT uint8_t lp_LDIRProofs_LDIR_payloadValid___lam__0(lean_object*, lean_object*);
+LEAN_EXPORT lean_object* lp_LDIRProofs_LDIR_payloadValid___lam__0___boxed(lean_object*, lean_object*);
+LEAN_EXPORT uint8_t lp_LDIRProofs_LDIR_payloadValid(lean_object*);
+LEAN_EXPORT lean_object* lp_LDIRProofs_LDIR_payloadValid___boxed(lean_object*);
 LEAN_EXPORT uint8_t lp_LDIRProofs_LDIR_wellFormedSIR(lean_object*);
 LEAN_EXPORT lean_object* lp_LDIRProofs_LDIR_wellFormedSIR___boxed(lean_object*);
+LEAN_EXPORT uint8_t lp_LDIRProofs_LDIR_wellFormedSIRWithPayload(lean_object*);
+LEAN_EXPORT lean_object* lp_LDIRProofs_LDIR_wellFormedSIRWithPayload___boxed(lean_object*);
 lean_object* lean_nat_add(lean_object*, lean_object*);
 LEAN_EXPORT uint8_t lp_LDIRProofs_LDIR_stackBalancedAux(lean_object*, lean_object*);
-uint8_t lean_nat_dec_lt(lean_object*, lean_object*);
-lean_object* lean_nat_sub(lean_object*, lean_object*);
 LEAN_EXPORT lean_object* lp_LDIRProofs_LDIR_stackBalancedAux___boxed(lean_object*, lean_object*);
 LEAN_EXPORT uint8_t lp_LDIRProofs_LDIR_stackBalanced(lean_object*);
 LEAN_EXPORT lean_object* lp_LDIRProofs_LDIR_stackBalanced___boxed(lean_object*);
@@ -364,6 +523,16 @@ LEAN_EXPORT lean_object* lp_LDIRProofs___private_LDIRProofs_proof__ir__wellforme
 LEAN_EXPORT lean_object* lp_LDIRProofs___private_LDIRProofs_proof__ir__wellformedness_0__LDIR_stackBalancedAux_match__1_splitter___redArg___boxed(lean_object*, lean_object*, lean_object*, lean_object*);
 LEAN_EXPORT lean_object* lp_LDIRProofs___private_LDIRProofs_proof__ir__wellformedness_0__LDIR_stackBalancedAux_match__1_splitter(lean_object*, uint8_t, lean_object*, lean_object*, lean_object*);
 LEAN_EXPORT lean_object* lp_LDIRProofs___private_LDIRProofs_proof__ir__wellformedness_0__LDIR_stackBalancedAux_match__1_splitter___boxed(lean_object*, lean_object*, lean_object*, lean_object*, lean_object*);
+LEAN_EXPORT lean_object* lp_LDIRProofs___private_LDIRProofs_proof__ir__wellformedness_0__List_any_match__1_splitter___redArg(lean_object*, lean_object*, lean_object*, lean_object*);
+LEAN_EXPORT lean_object* lp_LDIRProofs___private_LDIRProofs_proof__ir__wellformedness_0__List_any_match__1_splitter(lean_object*, lean_object*, lean_object*, lean_object*, lean_object*, lean_object*);
+LEAN_EXPORT lean_object* lp_LDIRProofs___private_LDIRProofs_proof__ir__wellformedness_0__LDIR_isAcyclicAux_match__3_splitter___redArg(lean_object*, lean_object*, lean_object*);
+LEAN_EXPORT lean_object* lp_LDIRProofs___private_LDIRProofs_proof__ir__wellformedness_0__LDIR_isAcyclicAux_match__3_splitter___redArg___boxed(lean_object*, lean_object*, lean_object*);
+LEAN_EXPORT lean_object* lp_LDIRProofs___private_LDIRProofs_proof__ir__wellformedness_0__LDIR_isAcyclicAux_match__3_splitter(lean_object*, lean_object*, lean_object*, lean_object*);
+LEAN_EXPORT lean_object* lp_LDIRProofs___private_LDIRProofs_proof__ir__wellformedness_0__LDIR_isAcyclicAux_match__3_splitter___boxed(lean_object*, lean_object*, lean_object*, lean_object*);
+LEAN_EXPORT lean_object* lp_LDIRProofs___private_LDIRProofs_proof__ir__wellformedness_0__LDIR_isAcyclicAux_match__1_splitter___redArg(lean_object*, lean_object*, lean_object*);
+LEAN_EXPORT lean_object* lp_LDIRProofs___private_LDIRProofs_proof__ir__wellformedness_0__LDIR_isAcyclicAux_match__1_splitter(lean_object*, lean_object*, lean_object*, lean_object*);
+LEAN_EXPORT lean_object* lp_LDIRProofs___private_LDIRProofs_proof__ir__wellformedness_0__LDIR_payloadValid_match__1_splitter___redArg(lean_object*, lean_object*, lean_object*);
+LEAN_EXPORT lean_object* lp_LDIRProofs___private_LDIRProofs_proof__ir__wellformedness_0__LDIR_payloadValid_match__1_splitter(lean_object*, lean_object*, lean_object*, lean_object*);
 LEAN_EXPORT lean_object* lp_LDIRProofs_LDIR_BlockType_ctorIdx(uint8_t x_1) {
 _start:
 {
@@ -398,11 +567,65 @@ lean_object* x_6;
 x_6 = lean_unsigned_to_nat(4u);
 return x_6;
 }
-default: 
+case 5:
 {
 lean_object* x_7; 
 x_7 = lean_unsigned_to_nat(5u);
 return x_7;
+}
+case 6:
+{
+lean_object* x_8; 
+x_8 = lean_unsigned_to_nat(6u);
+return x_8;
+}
+case 7:
+{
+lean_object* x_9; 
+x_9 = lean_unsigned_to_nat(7u);
+return x_9;
+}
+case 8:
+{
+lean_object* x_10; 
+x_10 = lean_unsigned_to_nat(8u);
+return x_10;
+}
+case 9:
+{
+lean_object* x_11; 
+x_11 = lean_unsigned_to_nat(9u);
+return x_11;
+}
+case 10:
+{
+lean_object* x_12; 
+x_12 = lean_unsigned_to_nat(10u);
+return x_12;
+}
+case 11:
+{
+lean_object* x_13; 
+x_13 = lean_unsigned_to_nat(11u);
+return x_13;
+}
+case 12:
+{
+lean_object* x_14; 
+x_14 = lean_unsigned_to_nat(12u);
+return x_14;
+}
+case 13:
+{
+lean_object* x_15; 
+x_15 = lean_unsigned_to_nat(13u);
+return x_15;
+}
+default: 
+{
+lean_object* x_16; 
+x_16 = lean_unsigned_to_nat(14u);
+return x_16;
 }
 }
 }
@@ -665,7 +888,304 @@ lean_dec(x_4);
 return x_6;
 }
 }
-static lean_object* _init_lp_LDIRProofs_LDIR_instReprBlockType_repr___closed__12(void) {
+LEAN_EXPORT lean_object* lp_LDIRProofs_LDIR_BlockType_blockQuote_elim___redArg(lean_object* x_1) {
+_start:
+{
+lean_inc(x_1);
+return x_1;
+}
+}
+LEAN_EXPORT lean_object* lp_LDIRProofs_LDIR_BlockType_blockQuote_elim___redArg___boxed(lean_object* x_1) {
+_start:
+{
+lean_object* x_2; 
+x_2 = lp_LDIRProofs_LDIR_BlockType_blockQuote_elim___redArg(x_1);
+lean_dec(x_1);
+return x_2;
+}
+}
+LEAN_EXPORT lean_object* lp_LDIRProofs_LDIR_BlockType_blockQuote_elim(lean_object* x_1, uint8_t x_2, lean_object* x_3, lean_object* x_4) {
+_start:
+{
+lean_inc(x_4);
+return x_4;
+}
+}
+LEAN_EXPORT lean_object* lp_LDIRProofs_LDIR_BlockType_blockQuote_elim___boxed(lean_object* x_1, lean_object* x_2, lean_object* x_3, lean_object* x_4) {
+_start:
+{
+uint8_t x_5; lean_object* x_6; 
+x_5 = lean_unbox(x_2);
+x_6 = lp_LDIRProofs_LDIR_BlockType_blockQuote_elim(x_1, x_5, x_3, x_4);
+lean_dec(x_4);
+return x_6;
+}
+}
+LEAN_EXPORT lean_object* lp_LDIRProofs_LDIR_BlockType_thematicBreak_elim___redArg(lean_object* x_1) {
+_start:
+{
+lean_inc(x_1);
+return x_1;
+}
+}
+LEAN_EXPORT lean_object* lp_LDIRProofs_LDIR_BlockType_thematicBreak_elim___redArg___boxed(lean_object* x_1) {
+_start:
+{
+lean_object* x_2; 
+x_2 = lp_LDIRProofs_LDIR_BlockType_thematicBreak_elim___redArg(x_1);
+lean_dec(x_1);
+return x_2;
+}
+}
+LEAN_EXPORT lean_object* lp_LDIRProofs_LDIR_BlockType_thematicBreak_elim(lean_object* x_1, uint8_t x_2, lean_object* x_3, lean_object* x_4) {
+_start:
+{
+lean_inc(x_4);
+return x_4;
+}
+}
+LEAN_EXPORT lean_object* lp_LDIRProofs_LDIR_BlockType_thematicBreak_elim___boxed(lean_object* x_1, lean_object* x_2, lean_object* x_3, lean_object* x_4) {
+_start:
+{
+uint8_t x_5; lean_object* x_6; 
+x_5 = lean_unbox(x_2);
+x_6 = lp_LDIRProofs_LDIR_BlockType_thematicBreak_elim(x_1, x_5, x_3, x_4);
+lean_dec(x_4);
+return x_6;
+}
+}
+LEAN_EXPORT lean_object* lp_LDIRProofs_LDIR_BlockType_image_elim___redArg(lean_object* x_1) {
+_start:
+{
+lean_inc(x_1);
+return x_1;
+}
+}
+LEAN_EXPORT lean_object* lp_LDIRProofs_LDIR_BlockType_image_elim___redArg___boxed(lean_object* x_1) {
+_start:
+{
+lean_object* x_2; 
+x_2 = lp_LDIRProofs_LDIR_BlockType_image_elim___redArg(x_1);
+lean_dec(x_1);
+return x_2;
+}
+}
+LEAN_EXPORT lean_object* lp_LDIRProofs_LDIR_BlockType_image_elim(lean_object* x_1, uint8_t x_2, lean_object* x_3, lean_object* x_4) {
+_start:
+{
+lean_inc(x_4);
+return x_4;
+}
+}
+LEAN_EXPORT lean_object* lp_LDIRProofs_LDIR_BlockType_image_elim___boxed(lean_object* x_1, lean_object* x_2, lean_object* x_3, lean_object* x_4) {
+_start:
+{
+uint8_t x_5; lean_object* x_6; 
+x_5 = lean_unbox(x_2);
+x_6 = lp_LDIRProofs_LDIR_BlockType_image_elim(x_1, x_5, x_3, x_4);
+lean_dec(x_4);
+return x_6;
+}
+}
+LEAN_EXPORT lean_object* lp_LDIRProofs_LDIR_BlockType_table_elim___redArg(lean_object* x_1) {
+_start:
+{
+lean_inc(x_1);
+return x_1;
+}
+}
+LEAN_EXPORT lean_object* lp_LDIRProofs_LDIR_BlockType_table_elim___redArg___boxed(lean_object* x_1) {
+_start:
+{
+lean_object* x_2; 
+x_2 = lp_LDIRProofs_LDIR_BlockType_table_elim___redArg(x_1);
+lean_dec(x_1);
+return x_2;
+}
+}
+LEAN_EXPORT lean_object* lp_LDIRProofs_LDIR_BlockType_table_elim(lean_object* x_1, uint8_t x_2, lean_object* x_3, lean_object* x_4) {
+_start:
+{
+lean_inc(x_4);
+return x_4;
+}
+}
+LEAN_EXPORT lean_object* lp_LDIRProofs_LDIR_BlockType_table_elim___boxed(lean_object* x_1, lean_object* x_2, lean_object* x_3, lean_object* x_4) {
+_start:
+{
+uint8_t x_5; lean_object* x_6; 
+x_5 = lean_unbox(x_2);
+x_6 = lp_LDIRProofs_LDIR_BlockType_table_elim(x_1, x_5, x_3, x_4);
+lean_dec(x_4);
+return x_6;
+}
+}
+LEAN_EXPORT lean_object* lp_LDIRProofs_LDIR_BlockType_tableRow_elim___redArg(lean_object* x_1) {
+_start:
+{
+lean_inc(x_1);
+return x_1;
+}
+}
+LEAN_EXPORT lean_object* lp_LDIRProofs_LDIR_BlockType_tableRow_elim___redArg___boxed(lean_object* x_1) {
+_start:
+{
+lean_object* x_2; 
+x_2 = lp_LDIRProofs_LDIR_BlockType_tableRow_elim___redArg(x_1);
+lean_dec(x_1);
+return x_2;
+}
+}
+LEAN_EXPORT lean_object* lp_LDIRProofs_LDIR_BlockType_tableRow_elim(lean_object* x_1, uint8_t x_2, lean_object* x_3, lean_object* x_4) {
+_start:
+{
+lean_inc(x_4);
+return x_4;
+}
+}
+LEAN_EXPORT lean_object* lp_LDIRProofs_LDIR_BlockType_tableRow_elim___boxed(lean_object* x_1, lean_object* x_2, lean_object* x_3, lean_object* x_4) {
+_start:
+{
+uint8_t x_5; lean_object* x_6; 
+x_5 = lean_unbox(x_2);
+x_6 = lp_LDIRProofs_LDIR_BlockType_tableRow_elim(x_1, x_5, x_3, x_4);
+lean_dec(x_4);
+return x_6;
+}
+}
+LEAN_EXPORT lean_object* lp_LDIRProofs_LDIR_BlockType_tableCell_elim___redArg(lean_object* x_1) {
+_start:
+{
+lean_inc(x_1);
+return x_1;
+}
+}
+LEAN_EXPORT lean_object* lp_LDIRProofs_LDIR_BlockType_tableCell_elim___redArg___boxed(lean_object* x_1) {
+_start:
+{
+lean_object* x_2; 
+x_2 = lp_LDIRProofs_LDIR_BlockType_tableCell_elim___redArg(x_1);
+lean_dec(x_1);
+return x_2;
+}
+}
+LEAN_EXPORT lean_object* lp_LDIRProofs_LDIR_BlockType_tableCell_elim(lean_object* x_1, uint8_t x_2, lean_object* x_3, lean_object* x_4) {
+_start:
+{
+lean_inc(x_4);
+return x_4;
+}
+}
+LEAN_EXPORT lean_object* lp_LDIRProofs_LDIR_BlockType_tableCell_elim___boxed(lean_object* x_1, lean_object* x_2, lean_object* x_3, lean_object* x_4) {
+_start:
+{
+uint8_t x_5; lean_object* x_6; 
+x_5 = lean_unbox(x_2);
+x_6 = lp_LDIRProofs_LDIR_BlockType_tableCell_elim(x_1, x_5, x_3, x_4);
+lean_dec(x_4);
+return x_6;
+}
+}
+LEAN_EXPORT lean_object* lp_LDIRProofs_LDIR_BlockType_footnote_elim___redArg(lean_object* x_1) {
+_start:
+{
+lean_inc(x_1);
+return x_1;
+}
+}
+LEAN_EXPORT lean_object* lp_LDIRProofs_LDIR_BlockType_footnote_elim___redArg___boxed(lean_object* x_1) {
+_start:
+{
+lean_object* x_2; 
+x_2 = lp_LDIRProofs_LDIR_BlockType_footnote_elim___redArg(x_1);
+lean_dec(x_1);
+return x_2;
+}
+}
+LEAN_EXPORT lean_object* lp_LDIRProofs_LDIR_BlockType_footnote_elim(lean_object* x_1, uint8_t x_2, lean_object* x_3, lean_object* x_4) {
+_start:
+{
+lean_inc(x_4);
+return x_4;
+}
+}
+LEAN_EXPORT lean_object* lp_LDIRProofs_LDIR_BlockType_footnote_elim___boxed(lean_object* x_1, lean_object* x_2, lean_object* x_3, lean_object* x_4) {
+_start:
+{
+uint8_t x_5; lean_object* x_6; 
+x_5 = lean_unbox(x_2);
+x_6 = lp_LDIRProofs_LDIR_BlockType_footnote_elim(x_1, x_5, x_3, x_4);
+lean_dec(x_4);
+return x_6;
+}
+}
+LEAN_EXPORT lean_object* lp_LDIRProofs_LDIR_BlockType_footnoteBlock_elim___redArg(lean_object* x_1) {
+_start:
+{
+lean_inc(x_1);
+return x_1;
+}
+}
+LEAN_EXPORT lean_object* lp_LDIRProofs_LDIR_BlockType_footnoteBlock_elim___redArg___boxed(lean_object* x_1) {
+_start:
+{
+lean_object* x_2; 
+x_2 = lp_LDIRProofs_LDIR_BlockType_footnoteBlock_elim___redArg(x_1);
+lean_dec(x_1);
+return x_2;
+}
+}
+LEAN_EXPORT lean_object* lp_LDIRProofs_LDIR_BlockType_footnoteBlock_elim(lean_object* x_1, uint8_t x_2, lean_object* x_3, lean_object* x_4) {
+_start:
+{
+lean_inc(x_4);
+return x_4;
+}
+}
+LEAN_EXPORT lean_object* lp_LDIRProofs_LDIR_BlockType_footnoteBlock_elim___boxed(lean_object* x_1, lean_object* x_2, lean_object* x_3, lean_object* x_4) {
+_start:
+{
+uint8_t x_5; lean_object* x_6; 
+x_5 = lean_unbox(x_2);
+x_6 = lp_LDIRProofs_LDIR_BlockType_footnoteBlock_elim(x_1, x_5, x_3, x_4);
+lean_dec(x_4);
+return x_6;
+}
+}
+LEAN_EXPORT lean_object* lp_LDIRProofs_LDIR_BlockType_figure_elim___redArg(lean_object* x_1) {
+_start:
+{
+lean_inc(x_1);
+return x_1;
+}
+}
+LEAN_EXPORT lean_object* lp_LDIRProofs_LDIR_BlockType_figure_elim___redArg___boxed(lean_object* x_1) {
+_start:
+{
+lean_object* x_2; 
+x_2 = lp_LDIRProofs_LDIR_BlockType_figure_elim___redArg(x_1);
+lean_dec(x_1);
+return x_2;
+}
+}
+LEAN_EXPORT lean_object* lp_LDIRProofs_LDIR_BlockType_figure_elim(lean_object* x_1, uint8_t x_2, lean_object* x_3, lean_object* x_4) {
+_start:
+{
+lean_inc(x_4);
+return x_4;
+}
+}
+LEAN_EXPORT lean_object* lp_LDIRProofs_LDIR_BlockType_figure_elim___boxed(lean_object* x_1, lean_object* x_2, lean_object* x_3, lean_object* x_4) {
+_start:
+{
+uint8_t x_5; lean_object* x_6; 
+x_5 = lean_unbox(x_2);
+x_6 = lp_LDIRProofs_LDIR_BlockType_figure_elim(x_1, x_5, x_3, x_4);
+lean_dec(x_4);
+return x_6;
+}
+}
+static lean_object* _init_lp_LDIRProofs_LDIR_instReprBlockType_repr___closed__30(void) {
 _start:
 {
 lean_object* x_1; lean_object* x_2; 
@@ -674,7 +1194,7 @@ x_2 = lean_nat_to_int(x_1);
 return x_2;
 }
 }
-static lean_object* _init_lp_LDIRProofs_LDIR_instReprBlockType_repr___closed__13(void) {
+static lean_object* _init_lp_LDIRProofs_LDIR_instReprBlockType_repr___closed__31(void) {
 _start:
 {
 lean_object* x_1; lean_object* x_2; 
@@ -686,126 +1206,306 @@ return x_2;
 LEAN_EXPORT lean_object* lp_LDIRProofs_LDIR_instReprBlockType_repr(uint8_t x_1, lean_object* x_2) {
 _start:
 {
-lean_object* x_3; lean_object* x_10; lean_object* x_17; lean_object* x_24; lean_object* x_31; lean_object* x_38; 
+lean_object* x_3; lean_object* x_10; lean_object* x_17; lean_object* x_24; lean_object* x_31; lean_object* x_38; lean_object* x_45; lean_object* x_52; lean_object* x_59; lean_object* x_66; lean_object* x_73; lean_object* x_80; lean_object* x_87; lean_object* x_94; lean_object* x_101; 
 switch (x_1) {
 case 0:
 {
-lean_object* x_45; uint8_t x_46; 
-x_45 = lean_unsigned_to_nat(1024u);
-x_46 = lean_nat_dec_le(x_45, x_2);
-if (x_46 == 0)
+lean_object* x_108; uint8_t x_109; 
+x_108 = lean_unsigned_to_nat(1024u);
+x_109 = lean_nat_dec_le(x_108, x_2);
+if (x_109 == 0)
 {
-lean_object* x_47; 
-x_47 = lean_obj_once(&lp_LDIRProofs_LDIR_instReprBlockType_repr___closed__12, &lp_LDIRProofs_LDIR_instReprBlockType_repr___closed__12_once, _init_lp_LDIRProofs_LDIR_instReprBlockType_repr___closed__12);
-x_3 = x_47;
+lean_object* x_110; 
+x_110 = lean_obj_once(&lp_LDIRProofs_LDIR_instReprBlockType_repr___closed__30, &lp_LDIRProofs_LDIR_instReprBlockType_repr___closed__30_once, _init_lp_LDIRProofs_LDIR_instReprBlockType_repr___closed__30);
+x_3 = x_110;
 goto block_9;
 }
 else
 {
-lean_object* x_48; 
-x_48 = lean_obj_once(&lp_LDIRProofs_LDIR_instReprBlockType_repr___closed__13, &lp_LDIRProofs_LDIR_instReprBlockType_repr___closed__13_once, _init_lp_LDIRProofs_LDIR_instReprBlockType_repr___closed__13);
-x_3 = x_48;
+lean_object* x_111; 
+x_111 = lean_obj_once(&lp_LDIRProofs_LDIR_instReprBlockType_repr___closed__31, &lp_LDIRProofs_LDIR_instReprBlockType_repr___closed__31_once, _init_lp_LDIRProofs_LDIR_instReprBlockType_repr___closed__31);
+x_3 = x_111;
 goto block_9;
 }
 }
 case 1:
 {
-lean_object* x_49; uint8_t x_50; 
-x_49 = lean_unsigned_to_nat(1024u);
-x_50 = lean_nat_dec_le(x_49, x_2);
-if (x_50 == 0)
+lean_object* x_112; uint8_t x_113; 
+x_112 = lean_unsigned_to_nat(1024u);
+x_113 = lean_nat_dec_le(x_112, x_2);
+if (x_113 == 0)
 {
-lean_object* x_51; 
-x_51 = lean_obj_once(&lp_LDIRProofs_LDIR_instReprBlockType_repr___closed__12, &lp_LDIRProofs_LDIR_instReprBlockType_repr___closed__12_once, _init_lp_LDIRProofs_LDIR_instReprBlockType_repr___closed__12);
-x_10 = x_51;
+lean_object* x_114; 
+x_114 = lean_obj_once(&lp_LDIRProofs_LDIR_instReprBlockType_repr___closed__30, &lp_LDIRProofs_LDIR_instReprBlockType_repr___closed__30_once, _init_lp_LDIRProofs_LDIR_instReprBlockType_repr___closed__30);
+x_10 = x_114;
 goto block_16;
 }
 else
 {
-lean_object* x_52; 
-x_52 = lean_obj_once(&lp_LDIRProofs_LDIR_instReprBlockType_repr___closed__13, &lp_LDIRProofs_LDIR_instReprBlockType_repr___closed__13_once, _init_lp_LDIRProofs_LDIR_instReprBlockType_repr___closed__13);
-x_10 = x_52;
+lean_object* x_115; 
+x_115 = lean_obj_once(&lp_LDIRProofs_LDIR_instReprBlockType_repr___closed__31, &lp_LDIRProofs_LDIR_instReprBlockType_repr___closed__31_once, _init_lp_LDIRProofs_LDIR_instReprBlockType_repr___closed__31);
+x_10 = x_115;
 goto block_16;
 }
 }
 case 2:
 {
-lean_object* x_53; uint8_t x_54; 
-x_53 = lean_unsigned_to_nat(1024u);
-x_54 = lean_nat_dec_le(x_53, x_2);
-if (x_54 == 0)
+lean_object* x_116; uint8_t x_117; 
+x_116 = lean_unsigned_to_nat(1024u);
+x_117 = lean_nat_dec_le(x_116, x_2);
+if (x_117 == 0)
 {
-lean_object* x_55; 
-x_55 = lean_obj_once(&lp_LDIRProofs_LDIR_instReprBlockType_repr___closed__12, &lp_LDIRProofs_LDIR_instReprBlockType_repr___closed__12_once, _init_lp_LDIRProofs_LDIR_instReprBlockType_repr___closed__12);
-x_17 = x_55;
+lean_object* x_118; 
+x_118 = lean_obj_once(&lp_LDIRProofs_LDIR_instReprBlockType_repr___closed__30, &lp_LDIRProofs_LDIR_instReprBlockType_repr___closed__30_once, _init_lp_LDIRProofs_LDIR_instReprBlockType_repr___closed__30);
+x_17 = x_118;
 goto block_23;
 }
 else
 {
-lean_object* x_56; 
-x_56 = lean_obj_once(&lp_LDIRProofs_LDIR_instReprBlockType_repr___closed__13, &lp_LDIRProofs_LDIR_instReprBlockType_repr___closed__13_once, _init_lp_LDIRProofs_LDIR_instReprBlockType_repr___closed__13);
-x_17 = x_56;
+lean_object* x_119; 
+x_119 = lean_obj_once(&lp_LDIRProofs_LDIR_instReprBlockType_repr___closed__31, &lp_LDIRProofs_LDIR_instReprBlockType_repr___closed__31_once, _init_lp_LDIRProofs_LDIR_instReprBlockType_repr___closed__31);
+x_17 = x_119;
 goto block_23;
 }
 }
 case 3:
 {
-lean_object* x_57; uint8_t x_58; 
-x_57 = lean_unsigned_to_nat(1024u);
-x_58 = lean_nat_dec_le(x_57, x_2);
-if (x_58 == 0)
+lean_object* x_120; uint8_t x_121; 
+x_120 = lean_unsigned_to_nat(1024u);
+x_121 = lean_nat_dec_le(x_120, x_2);
+if (x_121 == 0)
 {
-lean_object* x_59; 
-x_59 = lean_obj_once(&lp_LDIRProofs_LDIR_instReprBlockType_repr___closed__12, &lp_LDIRProofs_LDIR_instReprBlockType_repr___closed__12_once, _init_lp_LDIRProofs_LDIR_instReprBlockType_repr___closed__12);
-x_24 = x_59;
+lean_object* x_122; 
+x_122 = lean_obj_once(&lp_LDIRProofs_LDIR_instReprBlockType_repr___closed__30, &lp_LDIRProofs_LDIR_instReprBlockType_repr___closed__30_once, _init_lp_LDIRProofs_LDIR_instReprBlockType_repr___closed__30);
+x_24 = x_122;
 goto block_30;
 }
 else
 {
-lean_object* x_60; 
-x_60 = lean_obj_once(&lp_LDIRProofs_LDIR_instReprBlockType_repr___closed__13, &lp_LDIRProofs_LDIR_instReprBlockType_repr___closed__13_once, _init_lp_LDIRProofs_LDIR_instReprBlockType_repr___closed__13);
-x_24 = x_60;
+lean_object* x_123; 
+x_123 = lean_obj_once(&lp_LDIRProofs_LDIR_instReprBlockType_repr___closed__31, &lp_LDIRProofs_LDIR_instReprBlockType_repr___closed__31_once, _init_lp_LDIRProofs_LDIR_instReprBlockType_repr___closed__31);
+x_24 = x_123;
 goto block_30;
 }
 }
 case 4:
 {
-lean_object* x_61; uint8_t x_62; 
-x_61 = lean_unsigned_to_nat(1024u);
-x_62 = lean_nat_dec_le(x_61, x_2);
-if (x_62 == 0)
+lean_object* x_124; uint8_t x_125; 
+x_124 = lean_unsigned_to_nat(1024u);
+x_125 = lean_nat_dec_le(x_124, x_2);
+if (x_125 == 0)
 {
-lean_object* x_63; 
-x_63 = lean_obj_once(&lp_LDIRProofs_LDIR_instReprBlockType_repr___closed__12, &lp_LDIRProofs_LDIR_instReprBlockType_repr___closed__12_once, _init_lp_LDIRProofs_LDIR_instReprBlockType_repr___closed__12);
-x_31 = x_63;
+lean_object* x_126; 
+x_126 = lean_obj_once(&lp_LDIRProofs_LDIR_instReprBlockType_repr___closed__30, &lp_LDIRProofs_LDIR_instReprBlockType_repr___closed__30_once, _init_lp_LDIRProofs_LDIR_instReprBlockType_repr___closed__30);
+x_31 = x_126;
 goto block_37;
 }
 else
 {
-lean_object* x_64; 
-x_64 = lean_obj_once(&lp_LDIRProofs_LDIR_instReprBlockType_repr___closed__13, &lp_LDIRProofs_LDIR_instReprBlockType_repr___closed__13_once, _init_lp_LDIRProofs_LDIR_instReprBlockType_repr___closed__13);
-x_31 = x_64;
+lean_object* x_127; 
+x_127 = lean_obj_once(&lp_LDIRProofs_LDIR_instReprBlockType_repr___closed__31, &lp_LDIRProofs_LDIR_instReprBlockType_repr___closed__31_once, _init_lp_LDIRProofs_LDIR_instReprBlockType_repr___closed__31);
+x_31 = x_127;
 goto block_37;
+}
+}
+case 5:
+{
+lean_object* x_128; uint8_t x_129; 
+x_128 = lean_unsigned_to_nat(1024u);
+x_129 = lean_nat_dec_le(x_128, x_2);
+if (x_129 == 0)
+{
+lean_object* x_130; 
+x_130 = lean_obj_once(&lp_LDIRProofs_LDIR_instReprBlockType_repr___closed__30, &lp_LDIRProofs_LDIR_instReprBlockType_repr___closed__30_once, _init_lp_LDIRProofs_LDIR_instReprBlockType_repr___closed__30);
+x_38 = x_130;
+goto block_44;
+}
+else
+{
+lean_object* x_131; 
+x_131 = lean_obj_once(&lp_LDIRProofs_LDIR_instReprBlockType_repr___closed__31, &lp_LDIRProofs_LDIR_instReprBlockType_repr___closed__31_once, _init_lp_LDIRProofs_LDIR_instReprBlockType_repr___closed__31);
+x_38 = x_131;
+goto block_44;
+}
+}
+case 6:
+{
+lean_object* x_132; uint8_t x_133; 
+x_132 = lean_unsigned_to_nat(1024u);
+x_133 = lean_nat_dec_le(x_132, x_2);
+if (x_133 == 0)
+{
+lean_object* x_134; 
+x_134 = lean_obj_once(&lp_LDIRProofs_LDIR_instReprBlockType_repr___closed__30, &lp_LDIRProofs_LDIR_instReprBlockType_repr___closed__30_once, _init_lp_LDIRProofs_LDIR_instReprBlockType_repr___closed__30);
+x_45 = x_134;
+goto block_51;
+}
+else
+{
+lean_object* x_135; 
+x_135 = lean_obj_once(&lp_LDIRProofs_LDIR_instReprBlockType_repr___closed__31, &lp_LDIRProofs_LDIR_instReprBlockType_repr___closed__31_once, _init_lp_LDIRProofs_LDIR_instReprBlockType_repr___closed__31);
+x_45 = x_135;
+goto block_51;
+}
+}
+case 7:
+{
+lean_object* x_136; uint8_t x_137; 
+x_136 = lean_unsigned_to_nat(1024u);
+x_137 = lean_nat_dec_le(x_136, x_2);
+if (x_137 == 0)
+{
+lean_object* x_138; 
+x_138 = lean_obj_once(&lp_LDIRProofs_LDIR_instReprBlockType_repr___closed__30, &lp_LDIRProofs_LDIR_instReprBlockType_repr___closed__30_once, _init_lp_LDIRProofs_LDIR_instReprBlockType_repr___closed__30);
+x_52 = x_138;
+goto block_58;
+}
+else
+{
+lean_object* x_139; 
+x_139 = lean_obj_once(&lp_LDIRProofs_LDIR_instReprBlockType_repr___closed__31, &lp_LDIRProofs_LDIR_instReprBlockType_repr___closed__31_once, _init_lp_LDIRProofs_LDIR_instReprBlockType_repr___closed__31);
+x_52 = x_139;
+goto block_58;
+}
+}
+case 8:
+{
+lean_object* x_140; uint8_t x_141; 
+x_140 = lean_unsigned_to_nat(1024u);
+x_141 = lean_nat_dec_le(x_140, x_2);
+if (x_141 == 0)
+{
+lean_object* x_142; 
+x_142 = lean_obj_once(&lp_LDIRProofs_LDIR_instReprBlockType_repr___closed__30, &lp_LDIRProofs_LDIR_instReprBlockType_repr___closed__30_once, _init_lp_LDIRProofs_LDIR_instReprBlockType_repr___closed__30);
+x_59 = x_142;
+goto block_65;
+}
+else
+{
+lean_object* x_143; 
+x_143 = lean_obj_once(&lp_LDIRProofs_LDIR_instReprBlockType_repr___closed__31, &lp_LDIRProofs_LDIR_instReprBlockType_repr___closed__31_once, _init_lp_LDIRProofs_LDIR_instReprBlockType_repr___closed__31);
+x_59 = x_143;
+goto block_65;
+}
+}
+case 9:
+{
+lean_object* x_144; uint8_t x_145; 
+x_144 = lean_unsigned_to_nat(1024u);
+x_145 = lean_nat_dec_le(x_144, x_2);
+if (x_145 == 0)
+{
+lean_object* x_146; 
+x_146 = lean_obj_once(&lp_LDIRProofs_LDIR_instReprBlockType_repr___closed__30, &lp_LDIRProofs_LDIR_instReprBlockType_repr___closed__30_once, _init_lp_LDIRProofs_LDIR_instReprBlockType_repr___closed__30);
+x_66 = x_146;
+goto block_72;
+}
+else
+{
+lean_object* x_147; 
+x_147 = lean_obj_once(&lp_LDIRProofs_LDIR_instReprBlockType_repr___closed__31, &lp_LDIRProofs_LDIR_instReprBlockType_repr___closed__31_once, _init_lp_LDIRProofs_LDIR_instReprBlockType_repr___closed__31);
+x_66 = x_147;
+goto block_72;
+}
+}
+case 10:
+{
+lean_object* x_148; uint8_t x_149; 
+x_148 = lean_unsigned_to_nat(1024u);
+x_149 = lean_nat_dec_le(x_148, x_2);
+if (x_149 == 0)
+{
+lean_object* x_150; 
+x_150 = lean_obj_once(&lp_LDIRProofs_LDIR_instReprBlockType_repr___closed__30, &lp_LDIRProofs_LDIR_instReprBlockType_repr___closed__30_once, _init_lp_LDIRProofs_LDIR_instReprBlockType_repr___closed__30);
+x_73 = x_150;
+goto block_79;
+}
+else
+{
+lean_object* x_151; 
+x_151 = lean_obj_once(&lp_LDIRProofs_LDIR_instReprBlockType_repr___closed__31, &lp_LDIRProofs_LDIR_instReprBlockType_repr___closed__31_once, _init_lp_LDIRProofs_LDIR_instReprBlockType_repr___closed__31);
+x_73 = x_151;
+goto block_79;
+}
+}
+case 11:
+{
+lean_object* x_152; uint8_t x_153; 
+x_152 = lean_unsigned_to_nat(1024u);
+x_153 = lean_nat_dec_le(x_152, x_2);
+if (x_153 == 0)
+{
+lean_object* x_154; 
+x_154 = lean_obj_once(&lp_LDIRProofs_LDIR_instReprBlockType_repr___closed__30, &lp_LDIRProofs_LDIR_instReprBlockType_repr___closed__30_once, _init_lp_LDIRProofs_LDIR_instReprBlockType_repr___closed__30);
+x_80 = x_154;
+goto block_86;
+}
+else
+{
+lean_object* x_155; 
+x_155 = lean_obj_once(&lp_LDIRProofs_LDIR_instReprBlockType_repr___closed__31, &lp_LDIRProofs_LDIR_instReprBlockType_repr___closed__31_once, _init_lp_LDIRProofs_LDIR_instReprBlockType_repr___closed__31);
+x_80 = x_155;
+goto block_86;
+}
+}
+case 12:
+{
+lean_object* x_156; uint8_t x_157; 
+x_156 = lean_unsigned_to_nat(1024u);
+x_157 = lean_nat_dec_le(x_156, x_2);
+if (x_157 == 0)
+{
+lean_object* x_158; 
+x_158 = lean_obj_once(&lp_LDIRProofs_LDIR_instReprBlockType_repr___closed__30, &lp_LDIRProofs_LDIR_instReprBlockType_repr___closed__30_once, _init_lp_LDIRProofs_LDIR_instReprBlockType_repr___closed__30);
+x_87 = x_158;
+goto block_93;
+}
+else
+{
+lean_object* x_159; 
+x_159 = lean_obj_once(&lp_LDIRProofs_LDIR_instReprBlockType_repr___closed__31, &lp_LDIRProofs_LDIR_instReprBlockType_repr___closed__31_once, _init_lp_LDIRProofs_LDIR_instReprBlockType_repr___closed__31);
+x_87 = x_159;
+goto block_93;
+}
+}
+case 13:
+{
+lean_object* x_160; uint8_t x_161; 
+x_160 = lean_unsigned_to_nat(1024u);
+x_161 = lean_nat_dec_le(x_160, x_2);
+if (x_161 == 0)
+{
+lean_object* x_162; 
+x_162 = lean_obj_once(&lp_LDIRProofs_LDIR_instReprBlockType_repr___closed__30, &lp_LDIRProofs_LDIR_instReprBlockType_repr___closed__30_once, _init_lp_LDIRProofs_LDIR_instReprBlockType_repr___closed__30);
+x_94 = x_162;
+goto block_100;
+}
+else
+{
+lean_object* x_163; 
+x_163 = lean_obj_once(&lp_LDIRProofs_LDIR_instReprBlockType_repr___closed__31, &lp_LDIRProofs_LDIR_instReprBlockType_repr___closed__31_once, _init_lp_LDIRProofs_LDIR_instReprBlockType_repr___closed__31);
+x_94 = x_163;
+goto block_100;
 }
 }
 default: 
 {
-lean_object* x_65; uint8_t x_66; 
-x_65 = lean_unsigned_to_nat(1024u);
-x_66 = lean_nat_dec_le(x_65, x_2);
-if (x_66 == 0)
+lean_object* x_164; uint8_t x_165; 
+x_164 = lean_unsigned_to_nat(1024u);
+x_165 = lean_nat_dec_le(x_164, x_2);
+if (x_165 == 0)
 {
-lean_object* x_67; 
-x_67 = lean_obj_once(&lp_LDIRProofs_LDIR_instReprBlockType_repr___closed__12, &lp_LDIRProofs_LDIR_instReprBlockType_repr___closed__12_once, _init_lp_LDIRProofs_LDIR_instReprBlockType_repr___closed__12);
-x_38 = x_67;
-goto block_44;
+lean_object* x_166; 
+x_166 = lean_obj_once(&lp_LDIRProofs_LDIR_instReprBlockType_repr___closed__30, &lp_LDIRProofs_LDIR_instReprBlockType_repr___closed__30_once, _init_lp_LDIRProofs_LDIR_instReprBlockType_repr___closed__30);
+x_101 = x_166;
+goto block_107;
 }
 else
 {
-lean_object* x_68; 
-x_68 = lean_obj_once(&lp_LDIRProofs_LDIR_instReprBlockType_repr___closed__13, &lp_LDIRProofs_LDIR_instReprBlockType_repr___closed__13_once, _init_lp_LDIRProofs_LDIR_instReprBlockType_repr___closed__13);
-x_38 = x_68;
-goto block_44;
+lean_object* x_167; 
+x_167 = lean_obj_once(&lp_LDIRProofs_LDIR_instReprBlockType_repr___closed__31, &lp_LDIRProofs_LDIR_instReprBlockType_repr___closed__31_once, _init_lp_LDIRProofs_LDIR_instReprBlockType_repr___closed__31);
+x_101 = x_167;
+goto block_107;
 }
 }
 }
@@ -893,6 +1593,132 @@ lean_ctor_set_uint8(x_42, sizeof(void*)*1, x_41);
 x_43 = l_Repr_addAppParen(x_42, x_2);
 return x_43;
 }
+block_51:
+{
+lean_object* x_46; lean_object* x_47; uint8_t x_48; lean_object* x_49; lean_object* x_50; 
+x_46 = ((lean_object*)(lp_LDIRProofs_LDIR_instReprBlockType_repr___closed__13));
+x_47 = lean_alloc_ctor(4, 2, 0);
+lean_ctor_set(x_47, 0, x_45);
+lean_ctor_set(x_47, 1, x_46);
+x_48 = 0;
+x_49 = lean_alloc_ctor(6, 1, 1);
+lean_ctor_set(x_49, 0, x_47);
+lean_ctor_set_uint8(x_49, sizeof(void*)*1, x_48);
+x_50 = l_Repr_addAppParen(x_49, x_2);
+return x_50;
+}
+block_58:
+{
+lean_object* x_53; lean_object* x_54; uint8_t x_55; lean_object* x_56; lean_object* x_57; 
+x_53 = ((lean_object*)(lp_LDIRProofs_LDIR_instReprBlockType_repr___closed__15));
+x_54 = lean_alloc_ctor(4, 2, 0);
+lean_ctor_set(x_54, 0, x_52);
+lean_ctor_set(x_54, 1, x_53);
+x_55 = 0;
+x_56 = lean_alloc_ctor(6, 1, 1);
+lean_ctor_set(x_56, 0, x_54);
+lean_ctor_set_uint8(x_56, sizeof(void*)*1, x_55);
+x_57 = l_Repr_addAppParen(x_56, x_2);
+return x_57;
+}
+block_65:
+{
+lean_object* x_60; lean_object* x_61; uint8_t x_62; lean_object* x_63; lean_object* x_64; 
+x_60 = ((lean_object*)(lp_LDIRProofs_LDIR_instReprBlockType_repr___closed__17));
+x_61 = lean_alloc_ctor(4, 2, 0);
+lean_ctor_set(x_61, 0, x_59);
+lean_ctor_set(x_61, 1, x_60);
+x_62 = 0;
+x_63 = lean_alloc_ctor(6, 1, 1);
+lean_ctor_set(x_63, 0, x_61);
+lean_ctor_set_uint8(x_63, sizeof(void*)*1, x_62);
+x_64 = l_Repr_addAppParen(x_63, x_2);
+return x_64;
+}
+block_72:
+{
+lean_object* x_67; lean_object* x_68; uint8_t x_69; lean_object* x_70; lean_object* x_71; 
+x_67 = ((lean_object*)(lp_LDIRProofs_LDIR_instReprBlockType_repr___closed__19));
+x_68 = lean_alloc_ctor(4, 2, 0);
+lean_ctor_set(x_68, 0, x_66);
+lean_ctor_set(x_68, 1, x_67);
+x_69 = 0;
+x_70 = lean_alloc_ctor(6, 1, 1);
+lean_ctor_set(x_70, 0, x_68);
+lean_ctor_set_uint8(x_70, sizeof(void*)*1, x_69);
+x_71 = l_Repr_addAppParen(x_70, x_2);
+return x_71;
+}
+block_79:
+{
+lean_object* x_74; lean_object* x_75; uint8_t x_76; lean_object* x_77; lean_object* x_78; 
+x_74 = ((lean_object*)(lp_LDIRProofs_LDIR_instReprBlockType_repr___closed__21));
+x_75 = lean_alloc_ctor(4, 2, 0);
+lean_ctor_set(x_75, 0, x_73);
+lean_ctor_set(x_75, 1, x_74);
+x_76 = 0;
+x_77 = lean_alloc_ctor(6, 1, 1);
+lean_ctor_set(x_77, 0, x_75);
+lean_ctor_set_uint8(x_77, sizeof(void*)*1, x_76);
+x_78 = l_Repr_addAppParen(x_77, x_2);
+return x_78;
+}
+block_86:
+{
+lean_object* x_81; lean_object* x_82; uint8_t x_83; lean_object* x_84; lean_object* x_85; 
+x_81 = ((lean_object*)(lp_LDIRProofs_LDIR_instReprBlockType_repr___closed__23));
+x_82 = lean_alloc_ctor(4, 2, 0);
+lean_ctor_set(x_82, 0, x_80);
+lean_ctor_set(x_82, 1, x_81);
+x_83 = 0;
+x_84 = lean_alloc_ctor(6, 1, 1);
+lean_ctor_set(x_84, 0, x_82);
+lean_ctor_set_uint8(x_84, sizeof(void*)*1, x_83);
+x_85 = l_Repr_addAppParen(x_84, x_2);
+return x_85;
+}
+block_93:
+{
+lean_object* x_88; lean_object* x_89; uint8_t x_90; lean_object* x_91; lean_object* x_92; 
+x_88 = ((lean_object*)(lp_LDIRProofs_LDIR_instReprBlockType_repr___closed__25));
+x_89 = lean_alloc_ctor(4, 2, 0);
+lean_ctor_set(x_89, 0, x_87);
+lean_ctor_set(x_89, 1, x_88);
+x_90 = 0;
+x_91 = lean_alloc_ctor(6, 1, 1);
+lean_ctor_set(x_91, 0, x_89);
+lean_ctor_set_uint8(x_91, sizeof(void*)*1, x_90);
+x_92 = l_Repr_addAppParen(x_91, x_2);
+return x_92;
+}
+block_100:
+{
+lean_object* x_95; lean_object* x_96; uint8_t x_97; lean_object* x_98; lean_object* x_99; 
+x_95 = ((lean_object*)(lp_LDIRProofs_LDIR_instReprBlockType_repr___closed__27));
+x_96 = lean_alloc_ctor(4, 2, 0);
+lean_ctor_set(x_96, 0, x_94);
+lean_ctor_set(x_96, 1, x_95);
+x_97 = 0;
+x_98 = lean_alloc_ctor(6, 1, 1);
+lean_ctor_set(x_98, 0, x_96);
+lean_ctor_set_uint8(x_98, sizeof(void*)*1, x_97);
+x_99 = l_Repr_addAppParen(x_98, x_2);
+return x_99;
+}
+block_107:
+{
+lean_object* x_102; lean_object* x_103; uint8_t x_104; lean_object* x_105; lean_object* x_106; 
+x_102 = ((lean_object*)(lp_LDIRProofs_LDIR_instReprBlockType_repr___closed__29));
+x_103 = lean_alloc_ctor(4, 2, 0);
+lean_ctor_set(x_103, 0, x_101);
+lean_ctor_set(x_103, 1, x_102);
+x_104 = 0;
+x_105 = lean_alloc_ctor(6, 1, 1);
+lean_ctor_set(x_105, 0, x_103);
+lean_ctor_set_uint8(x_105, sizeof(void*)*1, x_104);
+x_106 = l_Repr_addAppParen(x_105, x_2);
+return x_106;
+}
 }
 }
 LEAN_EXPORT lean_object* lp_LDIRProofs_LDIR_instReprBlockType_repr___boxed(lean_object* x_1, lean_object* x_2) {
@@ -932,66 +1758,174 @@ LEAN_EXPORT uint8_t lp_LDIRProofs_LDIR_BlockType_ofNat(lean_object* x_1) {
 _start:
 {
 lean_object* x_2; uint8_t x_3; 
-x_2 = lean_unsigned_to_nat(2u);
+x_2 = lean_unsigned_to_nat(6u);
 x_3 = lean_nat_dec_le(x_1, x_2);
 if (x_3 == 0)
 {
 lean_object* x_4; uint8_t x_5; 
-x_4 = lean_unsigned_to_nat(3u);
+x_4 = lean_unsigned_to_nat(10u);
 x_5 = lean_nat_dec_le(x_1, x_4);
 if (x_5 == 0)
 {
 lean_object* x_6; uint8_t x_7; 
-x_6 = lean_unsigned_to_nat(4u);
+x_6 = lean_unsigned_to_nat(12u);
 x_7 = lean_nat_dec_le(x_1, x_6);
 if (x_7 == 0)
 {
-uint8_t x_8; 
-x_8 = 5;
-return x_8;
-}
-else
-{
-uint8_t x_9; 
-x_9 = 4;
-return x_9;
-}
-}
-else
+lean_object* x_8; uint8_t x_9; 
+x_8 = lean_unsigned_to_nat(13u);
+x_9 = lean_nat_dec_le(x_1, x_8);
+if (x_9 == 0)
 {
 uint8_t x_10; 
-x_10 = 3;
+x_10 = 14;
 return x_10;
 }
+else
+{
+uint8_t x_11; 
+x_11 = 13;
+return x_11;
+}
 }
 else
 {
-lean_object* x_11; uint8_t x_12; 
-x_11 = lean_unsigned_to_nat(0u);
-x_12 = lean_nat_dec_le(x_1, x_11);
-if (x_12 == 0)
+lean_object* x_12; uint8_t x_13; 
+x_12 = lean_unsigned_to_nat(11u);
+x_13 = lean_nat_dec_le(x_1, x_12);
+if (x_13 == 0)
 {
-lean_object* x_13; uint8_t x_14; 
-x_13 = lean_unsigned_to_nat(1u);
-x_14 = lean_nat_dec_le(x_1, x_13);
-if (x_14 == 0)
+uint8_t x_14; 
+x_14 = 12;
+return x_14;
+}
+else
 {
 uint8_t x_15; 
-x_15 = 2;
+x_15 = 11;
 return x_15;
 }
-else
-{
-uint8_t x_16; 
-x_16 = 1;
-return x_16;
 }
 }
 else
 {
-uint8_t x_17; 
-x_17 = 0;
-return x_17;
+lean_object* x_16; uint8_t x_17; 
+x_16 = lean_unsigned_to_nat(8u);
+x_17 = lean_nat_dec_le(x_1, x_16);
+if (x_17 == 0)
+{
+lean_object* x_18; uint8_t x_19; 
+x_18 = lean_unsigned_to_nat(9u);
+x_19 = lean_nat_dec_le(x_1, x_18);
+if (x_19 == 0)
+{
+uint8_t x_20; 
+x_20 = 10;
+return x_20;
+}
+else
+{
+uint8_t x_21; 
+x_21 = 9;
+return x_21;
+}
+}
+else
+{
+lean_object* x_22; uint8_t x_23; 
+x_22 = lean_unsigned_to_nat(7u);
+x_23 = lean_nat_dec_le(x_1, x_22);
+if (x_23 == 0)
+{
+uint8_t x_24; 
+x_24 = 8;
+return x_24;
+}
+else
+{
+uint8_t x_25; 
+x_25 = 7;
+return x_25;
+}
+}
+}
+}
+else
+{
+lean_object* x_26; uint8_t x_27; 
+x_26 = lean_unsigned_to_nat(2u);
+x_27 = lean_nat_dec_le(x_1, x_26);
+if (x_27 == 0)
+{
+lean_object* x_28; uint8_t x_29; 
+x_28 = lean_unsigned_to_nat(4u);
+x_29 = lean_nat_dec_le(x_1, x_28);
+if (x_29 == 0)
+{
+lean_object* x_30; uint8_t x_31; 
+x_30 = lean_unsigned_to_nat(5u);
+x_31 = lean_nat_dec_le(x_1, x_30);
+if (x_31 == 0)
+{
+uint8_t x_32; 
+x_32 = 6;
+return x_32;
+}
+else
+{
+uint8_t x_33; 
+x_33 = 5;
+return x_33;
+}
+}
+else
+{
+lean_object* x_34; uint8_t x_35; 
+x_34 = lean_unsigned_to_nat(3u);
+x_35 = lean_nat_dec_le(x_1, x_34);
+if (x_35 == 0)
+{
+uint8_t x_36; 
+x_36 = 4;
+return x_36;
+}
+else
+{
+uint8_t x_37; 
+x_37 = 3;
+return x_37;
+}
+}
+}
+else
+{
+lean_object* x_38; uint8_t x_39; 
+x_38 = lean_unsigned_to_nat(0u);
+x_39 = lean_nat_dec_le(x_1, x_38);
+if (x_39 == 0)
+{
+lean_object* x_40; uint8_t x_41; 
+x_40 = lean_unsigned_to_nat(1u);
+x_41 = lean_nat_dec_le(x_1, x_40);
+if (x_41 == 0)
+{
+uint8_t x_42; 
+x_42 = 2;
+return x_42;
+}
+else
+{
+uint8_t x_43; 
+x_43 = 1;
+return x_43;
+}
+}
+else
+{
+uint8_t x_44; 
+x_44 = 0;
+return x_44;
+}
 }
 }
 }
@@ -1303,14 +2237,14 @@ x_43 = lean_nat_dec_le(x_42, x_2);
 if (x_43 == 0)
 {
 lean_object* x_44; 
-x_44 = lean_obj_once(&lp_LDIRProofs_LDIR_instReprBlockType_repr___closed__12, &lp_LDIRProofs_LDIR_instReprBlockType_repr___closed__12_once, _init_lp_LDIRProofs_LDIR_instReprBlockType_repr___closed__12);
+x_44 = lean_obj_once(&lp_LDIRProofs_LDIR_instReprBlockType_repr___closed__30, &lp_LDIRProofs_LDIR_instReprBlockType_repr___closed__30_once, _init_lp_LDIRProofs_LDIR_instReprBlockType_repr___closed__30);
 x_32 = x_44;
 goto block_41;
 }
 else
 {
 lean_object* x_45; 
-x_45 = lean_obj_once(&lp_LDIRProofs_LDIR_instReprBlockType_repr___closed__13, &lp_LDIRProofs_LDIR_instReprBlockType_repr___closed__13_once, _init_lp_LDIRProofs_LDIR_instReprBlockType_repr___closed__13);
+x_45 = lean_obj_once(&lp_LDIRProofs_LDIR_instReprBlockType_repr___closed__31, &lp_LDIRProofs_LDIR_instReprBlockType_repr___closed__31_once, _init_lp_LDIRProofs_LDIR_instReprBlockType_repr___closed__31);
 x_32 = x_45;
 goto block_41;
 }
@@ -1342,14 +2276,14 @@ x_47 = lean_nat_dec_le(x_46, x_2);
 if (x_47 == 0)
 {
 lean_object* x_48; 
-x_48 = lean_obj_once(&lp_LDIRProofs_LDIR_instReprBlockType_repr___closed__12, &lp_LDIRProofs_LDIR_instReprBlockType_repr___closed__12_once, _init_lp_LDIRProofs_LDIR_instReprBlockType_repr___closed__12);
+x_48 = lean_obj_once(&lp_LDIRProofs_LDIR_instReprBlockType_repr___closed__30, &lp_LDIRProofs_LDIR_instReprBlockType_repr___closed__30_once, _init_lp_LDIRProofs_LDIR_instReprBlockType_repr___closed__30);
 x_3 = x_48;
 goto block_9;
 }
 else
 {
 lean_object* x_49; 
-x_49 = lean_obj_once(&lp_LDIRProofs_LDIR_instReprBlockType_repr___closed__13, &lp_LDIRProofs_LDIR_instReprBlockType_repr___closed__13_once, _init_lp_LDIRProofs_LDIR_instReprBlockType_repr___closed__13);
+x_49 = lean_obj_once(&lp_LDIRProofs_LDIR_instReprBlockType_repr___closed__31, &lp_LDIRProofs_LDIR_instReprBlockType_repr___closed__31_once, _init_lp_LDIRProofs_LDIR_instReprBlockType_repr___closed__31);
 x_3 = x_49;
 goto block_9;
 }
@@ -1362,14 +2296,14 @@ x_51 = lean_nat_dec_le(x_50, x_2);
 if (x_51 == 0)
 {
 lean_object* x_52; 
-x_52 = lean_obj_once(&lp_LDIRProofs_LDIR_instReprBlockType_repr___closed__12, &lp_LDIRProofs_LDIR_instReprBlockType_repr___closed__12_once, _init_lp_LDIRProofs_LDIR_instReprBlockType_repr___closed__12);
+x_52 = lean_obj_once(&lp_LDIRProofs_LDIR_instReprBlockType_repr___closed__30, &lp_LDIRProofs_LDIR_instReprBlockType_repr___closed__30_once, _init_lp_LDIRProofs_LDIR_instReprBlockType_repr___closed__30);
 x_10 = x_52;
 goto block_16;
 }
 else
 {
 lean_object* x_53; 
-x_53 = lean_obj_once(&lp_LDIRProofs_LDIR_instReprBlockType_repr___closed__13, &lp_LDIRProofs_LDIR_instReprBlockType_repr___closed__13_once, _init_lp_LDIRProofs_LDIR_instReprBlockType_repr___closed__13);
+x_53 = lean_obj_once(&lp_LDIRProofs_LDIR_instReprBlockType_repr___closed__31, &lp_LDIRProofs_LDIR_instReprBlockType_repr___closed__31_once, _init_lp_LDIRProofs_LDIR_instReprBlockType_repr___closed__31);
 x_10 = x_53;
 goto block_16;
 }
@@ -1382,14 +2316,14 @@ x_55 = lean_nat_dec_le(x_54, x_2);
 if (x_55 == 0)
 {
 lean_object* x_56; 
-x_56 = lean_obj_once(&lp_LDIRProofs_LDIR_instReprBlockType_repr___closed__12, &lp_LDIRProofs_LDIR_instReprBlockType_repr___closed__12_once, _init_lp_LDIRProofs_LDIR_instReprBlockType_repr___closed__12);
+x_56 = lean_obj_once(&lp_LDIRProofs_LDIR_instReprBlockType_repr___closed__30, &lp_LDIRProofs_LDIR_instReprBlockType_repr___closed__30_once, _init_lp_LDIRProofs_LDIR_instReprBlockType_repr___closed__30);
 x_17 = x_56;
 goto block_23;
 }
 else
 {
 lean_object* x_57; 
-x_57 = lean_obj_once(&lp_LDIRProofs_LDIR_instReprBlockType_repr___closed__13, &lp_LDIRProofs_LDIR_instReprBlockType_repr___closed__13_once, _init_lp_LDIRProofs_LDIR_instReprBlockType_repr___closed__13);
+x_57 = lean_obj_once(&lp_LDIRProofs_LDIR_instReprBlockType_repr___closed__31, &lp_LDIRProofs_LDIR_instReprBlockType_repr___closed__31_once, _init_lp_LDIRProofs_LDIR_instReprBlockType_repr___closed__31);
 x_17 = x_57;
 goto block_23;
 }
@@ -1402,14 +2336,14 @@ x_59 = lean_nat_dec_le(x_58, x_2);
 if (x_59 == 0)
 {
 lean_object* x_60; 
-x_60 = lean_obj_once(&lp_LDIRProofs_LDIR_instReprBlockType_repr___closed__12, &lp_LDIRProofs_LDIR_instReprBlockType_repr___closed__12_once, _init_lp_LDIRProofs_LDIR_instReprBlockType_repr___closed__12);
+x_60 = lean_obj_once(&lp_LDIRProofs_LDIR_instReprBlockType_repr___closed__30, &lp_LDIRProofs_LDIR_instReprBlockType_repr___closed__30_once, _init_lp_LDIRProofs_LDIR_instReprBlockType_repr___closed__30);
 x_24 = x_60;
 goto block_30;
 }
 else
 {
 lean_object* x_61; 
-x_61 = lean_obj_once(&lp_LDIRProofs_LDIR_instReprBlockType_repr___closed__13, &lp_LDIRProofs_LDIR_instReprBlockType_repr___closed__13_once, _init_lp_LDIRProofs_LDIR_instReprBlockType_repr___closed__13);
+x_61 = lean_obj_once(&lp_LDIRProofs_LDIR_instReprBlockType_repr___closed__31, &lp_LDIRProofs_LDIR_instReprBlockType_repr___closed__31_once, _init_lp_LDIRProofs_LDIR_instReprBlockType_repr___closed__31);
 x_24 = x_61;
 goto block_30;
 }
@@ -1981,6 +2915,565 @@ x_4 = lean_box(x_3);
 return x_4;
 }
 }
+static lean_object* _init_lp_LDIRProofs_LDIR_instReprPayloadTable_repr___redArg___closed__4(void) {
+_start:
+{
+lean_object* x_1; lean_object* x_2; 
+x_1 = lean_unsigned_to_nat(8u);
+x_2 = lean_nat_to_int(x_1);
+return x_2;
+}
+}
+LEAN_EXPORT lean_object* lp_LDIRProofs_LDIR_instReprPayloadTable_repr___redArg(lean_object* x_1) {
+_start:
+{
+lean_object* x_2; lean_object* x_3; lean_object* x_4; lean_object* x_5; lean_object* x_6; uint8_t x_7; lean_object* x_8; lean_object* x_9; lean_object* x_10; lean_object* x_11; lean_object* x_12; lean_object* x_13; lean_object* x_14; lean_object* x_15; lean_object* x_16; 
+x_2 = ((lean_object*)(lp_LDIRProofs_LDIR_instReprPayloadTable_repr___redArg___closed__3));
+x_3 = lean_obj_once(&lp_LDIRProofs_LDIR_instReprPayloadTable_repr___redArg___closed__4, &lp_LDIRProofs_LDIR_instReprPayloadTable_repr___redArg___closed__4_once, _init_lp_LDIRProofs_LDIR_instReprPayloadTable_repr___redArg___closed__4);
+x_4 = l_String_quote(x_1);
+x_5 = lean_alloc_ctor(3, 1, 0);
+lean_ctor_set(x_5, 0, x_4);
+x_6 = lean_alloc_ctor(4, 2, 0);
+lean_ctor_set(x_6, 0, x_3);
+lean_ctor_set(x_6, 1, x_5);
+x_7 = 0;
+x_8 = lean_alloc_ctor(6, 1, 1);
+lean_ctor_set(x_8, 0, x_6);
+lean_ctor_set_uint8(x_8, sizeof(void*)*1, x_7);
+x_9 = lean_alloc_ctor(5, 2, 0);
+lean_ctor_set(x_9, 0, x_2);
+lean_ctor_set(x_9, 1, x_8);
+x_10 = lean_obj_once(&lp_LDIRProofs_LDIR_instReprSIRInstruction_repr___redArg___closed__20, &lp_LDIRProofs_LDIR_instReprSIRInstruction_repr___redArg___closed__20_once, _init_lp_LDIRProofs_LDIR_instReprSIRInstruction_repr___redArg___closed__20);
+x_11 = ((lean_object*)(lp_LDIRProofs_LDIR_instReprSIRInstruction_repr___redArg___closed__21));
+x_12 = lean_alloc_ctor(5, 2, 0);
+lean_ctor_set(x_12, 0, x_11);
+lean_ctor_set(x_12, 1, x_9);
+x_13 = ((lean_object*)(lp_LDIRProofs_LDIR_instReprSIRInstruction_repr___redArg___closed__22));
+x_14 = lean_alloc_ctor(5, 2, 0);
+lean_ctor_set(x_14, 0, x_12);
+lean_ctor_set(x_14, 1, x_13);
+x_15 = lean_alloc_ctor(4, 2, 0);
+lean_ctor_set(x_15, 0, x_10);
+lean_ctor_set(x_15, 1, x_14);
+x_16 = lean_alloc_ctor(6, 1, 1);
+lean_ctor_set(x_16, 0, x_15);
+lean_ctor_set_uint8(x_16, sizeof(void*)*1, x_7);
+return x_16;
+}
+}
+LEAN_EXPORT lean_object* lp_LDIRProofs_LDIR_instReprPayloadTable_repr(lean_object* x_1, lean_object* x_2) {
+_start:
+{
+lean_object* x_3; 
+x_3 = lp_LDIRProofs_LDIR_instReprPayloadTable_repr___redArg(x_1);
+return x_3;
+}
+}
+LEAN_EXPORT lean_object* lp_LDIRProofs_LDIR_instReprPayloadTable_repr___boxed(lean_object* x_1, lean_object* x_2) {
+_start:
+{
+lean_object* x_3; 
+x_3 = lp_LDIRProofs_LDIR_instReprPayloadTable_repr(x_1, x_2);
+lean_dec(x_2);
+return x_3;
+}
+}
+LEAN_EXPORT uint8_t lp_LDIRProofs_LDIR_instBEqPayloadTable_beq(lean_object* x_1, lean_object* x_2) {
+_start:
+{
+uint8_t x_3; 
+x_3 = lean_string_dec_eq(x_1, x_2);
+return x_3;
+}
+}
+LEAN_EXPORT lean_object* lp_LDIRProofs_LDIR_instBEqPayloadTable_beq___boxed(lean_object* x_1, lean_object* x_2) {
+_start:
+{
+uint8_t x_3; lean_object* x_4; 
+x_3 = lp_LDIRProofs_LDIR_instBEqPayloadTable_beq(x_1, x_2);
+lean_dec_ref(x_2);
+lean_dec_ref(x_1);
+x_4 = lean_box(x_3);
+return x_4;
+}
+}
+LEAN_EXPORT lean_object* lp_LDIRProofs_List_foldl___at___00List_foldl___at___00Std_Format_joinSep___at___00List_repr___at___00LDIR_instReprSIRDocumentWithPayload_repr_spec__0_spec__0_spec__1_spec__2(lean_object* x_1, lean_object* x_2, lean_object* x_3) {
+_start:
+{
+if (lean_obj_tag(x_3) == 0)
+{
+lean_dec(x_1);
+return x_2;
+}
+else
+{
+uint8_t x_4; 
+x_4 = !lean_is_exclusive(x_3);
+if (x_4 == 0)
+{
+lean_object* x_5; lean_object* x_6; lean_object* x_7; lean_object* x_8; 
+x_5 = lean_ctor_get(x_3, 0);
+x_6 = lean_ctor_get(x_3, 1);
+lean_inc(x_1);
+lean_ctor_set_tag(x_3, 5);
+lean_ctor_set(x_3, 1, x_1);
+lean_ctor_set(x_3, 0, x_2);
+x_7 = lp_LDIRProofs_LDIR_instReprSIRInstruction_repr___redArg(x_5);
+x_8 = lean_alloc_ctor(5, 2, 0);
+lean_ctor_set(x_8, 0, x_3);
+lean_ctor_set(x_8, 1, x_7);
+x_2 = x_8;
+x_3 = x_6;
+goto _start;
+}
+else
+{
+lean_object* x_10; lean_object* x_11; lean_object* x_12; lean_object* x_13; lean_object* x_14; 
+x_10 = lean_ctor_get(x_3, 0);
+x_11 = lean_ctor_get(x_3, 1);
+lean_inc(x_11);
+lean_inc(x_10);
+lean_dec(x_3);
+lean_inc(x_1);
+x_12 = lean_alloc_ctor(5, 2, 0);
+lean_ctor_set(x_12, 0, x_2);
+lean_ctor_set(x_12, 1, x_1);
+x_13 = lp_LDIRProofs_LDIR_instReprSIRInstruction_repr___redArg(x_10);
+x_14 = lean_alloc_ctor(5, 2, 0);
+lean_ctor_set(x_14, 0, x_12);
+lean_ctor_set(x_14, 1, x_13);
+x_2 = x_14;
+x_3 = x_11;
+goto _start;
+}
+}
+}
+}
+LEAN_EXPORT lean_object* lp_LDIRProofs_List_foldl___at___00Std_Format_joinSep___at___00List_repr___at___00LDIR_instReprSIRDocumentWithPayload_repr_spec__0_spec__0_spec__1(lean_object* x_1, lean_object* x_2, lean_object* x_3) {
+_start:
+{
+if (lean_obj_tag(x_3) == 0)
+{
+lean_dec(x_1);
+return x_2;
+}
+else
+{
+uint8_t x_4; 
+x_4 = !lean_is_exclusive(x_3);
+if (x_4 == 0)
+{
+lean_object* x_5; lean_object* x_6; lean_object* x_7; lean_object* x_8; lean_object* x_9; 
+x_5 = lean_ctor_get(x_3, 0);
+x_6 = lean_ctor_get(x_3, 1);
+lean_inc(x_1);
+lean_ctor_set_tag(x_3, 5);
+lean_ctor_set(x_3, 1, x_1);
+lean_ctor_set(x_3, 0, x_2);
+x_7 = lp_LDIRProofs_LDIR_instReprSIRInstruction_repr___redArg(x_5);
+x_8 = lean_alloc_ctor(5, 2, 0);
+lean_ctor_set(x_8, 0, x_3);
+lean_ctor_set(x_8, 1, x_7);
+x_9 = lp_LDIRProofs_List_foldl___at___00List_foldl___at___00Std_Format_joinSep___at___00List_repr___at___00LDIR_instReprSIRDocumentWithPayload_repr_spec__0_spec__0_spec__1_spec__2(x_1, x_8, x_6);
+return x_9;
+}
+else
+{
+lean_object* x_10; lean_object* x_11; lean_object* x_12; lean_object* x_13; lean_object* x_14; lean_object* x_15; 
+x_10 = lean_ctor_get(x_3, 0);
+x_11 = lean_ctor_get(x_3, 1);
+lean_inc(x_11);
+lean_inc(x_10);
+lean_dec(x_3);
+lean_inc(x_1);
+x_12 = lean_alloc_ctor(5, 2, 0);
+lean_ctor_set(x_12, 0, x_2);
+lean_ctor_set(x_12, 1, x_1);
+x_13 = lp_LDIRProofs_LDIR_instReprSIRInstruction_repr___redArg(x_10);
+x_14 = lean_alloc_ctor(5, 2, 0);
+lean_ctor_set(x_14, 0, x_12);
+lean_ctor_set(x_14, 1, x_13);
+x_15 = lp_LDIRProofs_List_foldl___at___00List_foldl___at___00Std_Format_joinSep___at___00List_repr___at___00LDIR_instReprSIRDocumentWithPayload_repr_spec__0_spec__0_spec__1_spec__2(x_1, x_14, x_11);
+return x_15;
+}
+}
+}
+}
+LEAN_EXPORT lean_object* lp_LDIRProofs_Std_Format_joinSep___at___00List_repr___at___00LDIR_instReprSIRDocumentWithPayload_repr_spec__0_spec__0(lean_object* x_1, lean_object* x_2) {
+_start:
+{
+if (lean_obj_tag(x_1) == 0)
+{
+lean_object* x_3; 
+lean_dec(x_2);
+x_3 = lean_box(0);
+return x_3;
+}
+else
+{
+lean_object* x_4; 
+x_4 = lean_ctor_get(x_1, 1);
+if (lean_obj_tag(x_4) == 0)
+{
+lean_object* x_5; lean_object* x_6; 
+lean_dec(x_2);
+x_5 = lean_ctor_get(x_1, 0);
+lean_inc(x_5);
+lean_dec_ref(x_1);
+x_6 = lp_LDIRProofs_LDIR_instReprSIRInstruction_repr___redArg(x_5);
+return x_6;
+}
+else
+{
+lean_object* x_7; lean_object* x_8; lean_object* x_9; 
+lean_inc(x_4);
+x_7 = lean_ctor_get(x_1, 0);
+lean_inc(x_7);
+lean_dec_ref(x_1);
+x_8 = lp_LDIRProofs_LDIR_instReprSIRInstruction_repr___redArg(x_7);
+x_9 = lp_LDIRProofs_List_foldl___at___00Std_Format_joinSep___at___00List_repr___at___00LDIR_instReprSIRDocumentWithPayload_repr_spec__0_spec__0_spec__1(x_2, x_8, x_4);
+return x_9;
+}
+}
+}
+}
+static lean_object* _init_lp_LDIRProofs_List_repr___at___00LDIR_instReprSIRDocumentWithPayload_repr_spec__0___redArg___closed__5(void) {
+_start:
+{
+lean_object* x_1; lean_object* x_2; 
+x_1 = ((lean_object*)(lp_LDIRProofs_List_repr___at___00LDIR_instReprSIRDocumentWithPayload_repr_spec__0___redArg___closed__2));
+x_2 = lean_string_length(x_1);
+return x_2;
+}
+}
+static lean_object* _init_lp_LDIRProofs_List_repr___at___00LDIR_instReprSIRDocumentWithPayload_repr_spec__0___redArg___closed__6(void) {
+_start:
+{
+lean_object* x_1; lean_object* x_2; 
+x_1 = lean_obj_once(&lp_LDIRProofs_List_repr___at___00LDIR_instReprSIRDocumentWithPayload_repr_spec__0___redArg___closed__5, &lp_LDIRProofs_List_repr___at___00LDIR_instReprSIRDocumentWithPayload_repr_spec__0___redArg___closed__5_once, _init_lp_LDIRProofs_List_repr___at___00LDIR_instReprSIRDocumentWithPayload_repr_spec__0___redArg___closed__5);
+x_2 = lean_nat_to_int(x_1);
+return x_2;
+}
+}
+LEAN_EXPORT lean_object* lp_LDIRProofs_List_repr___at___00LDIR_instReprSIRDocumentWithPayload_repr_spec__0___redArg(lean_object* x_1) {
+_start:
+{
+if (lean_obj_tag(x_1) == 0)
+{
+lean_object* x_2; 
+x_2 = ((lean_object*)(lp_LDIRProofs_List_repr___at___00LDIR_instReprSIRDocumentWithPayload_repr_spec__0___redArg___closed__1));
+return x_2;
+}
+else
+{
+lean_object* x_3; lean_object* x_4; lean_object* x_5; lean_object* x_6; lean_object* x_7; lean_object* x_8; lean_object* x_9; lean_object* x_10; uint8_t x_11; lean_object* x_12; 
+x_3 = ((lean_object*)(lp_LDIRProofs_List_repr___at___00LDIR_instReprSIRDocumentWithPayload_repr_spec__0___redArg___closed__3));
+x_4 = lp_LDIRProofs_Std_Format_joinSep___at___00List_repr___at___00LDIR_instReprSIRDocumentWithPayload_repr_spec__0_spec__0(x_1, x_3);
+x_5 = lean_obj_once(&lp_LDIRProofs_List_repr___at___00LDIR_instReprSIRDocumentWithPayload_repr_spec__0___redArg___closed__6, &lp_LDIRProofs_List_repr___at___00LDIR_instReprSIRDocumentWithPayload_repr_spec__0___redArg___closed__6_once, _init_lp_LDIRProofs_List_repr___at___00LDIR_instReprSIRDocumentWithPayload_repr_spec__0___redArg___closed__6);
+x_6 = ((lean_object*)(lp_LDIRProofs_List_repr___at___00LDIR_instReprSIRDocumentWithPayload_repr_spec__0___redArg___closed__7));
+x_7 = lean_alloc_ctor(5, 2, 0);
+lean_ctor_set(x_7, 0, x_6);
+lean_ctor_set(x_7, 1, x_4);
+x_8 = ((lean_object*)(lp_LDIRProofs_List_repr___at___00LDIR_instReprSIRDocumentWithPayload_repr_spec__0___redArg___closed__8));
+x_9 = lean_alloc_ctor(5, 2, 0);
+lean_ctor_set(x_9, 0, x_7);
+lean_ctor_set(x_9, 1, x_8);
+x_10 = lean_alloc_ctor(4, 2, 0);
+lean_ctor_set(x_10, 0, x_5);
+lean_ctor_set(x_10, 1, x_9);
+x_11 = 0;
+x_12 = lean_alloc_ctor(6, 1, 1);
+lean_ctor_set(x_12, 0, x_10);
+lean_ctor_set_uint8(x_12, sizeof(void*)*1, x_11);
+return x_12;
+}
+}
+}
+static lean_object* _init_lp_LDIRProofs_LDIR_instReprSIRDocumentWithPayload_repr___redArg___closed__4(void) {
+_start:
+{
+lean_object* x_1; lean_object* x_2; 
+x_1 = lean_unsigned_to_nat(16u);
+x_2 = lean_nat_to_int(x_1);
+return x_2;
+}
+}
+static lean_object* _init_lp_LDIRProofs_LDIR_instReprSIRDocumentWithPayload_repr___redArg___closed__7(void) {
+_start:
+{
+lean_object* x_1; lean_object* x_2; 
+x_1 = lean_unsigned_to_nat(11u);
+x_2 = lean_nat_to_int(x_1);
+return x_2;
+}
+}
+LEAN_EXPORT lean_object* lp_LDIRProofs_LDIR_instReprSIRDocumentWithPayload_repr___redArg(lean_object* x_1) {
+_start:
+{
+uint8_t x_2; 
+x_2 = !lean_is_exclusive(x_1);
+if (x_2 == 0)
+{
+lean_object* x_3; lean_object* x_4; lean_object* x_5; lean_object* x_6; lean_object* x_7; lean_object* x_8; uint8_t x_9; lean_object* x_10; lean_object* x_11; lean_object* x_12; lean_object* x_13; lean_object* x_14; lean_object* x_15; lean_object* x_16; lean_object* x_17; lean_object* x_18; lean_object* x_19; lean_object* x_20; lean_object* x_21; lean_object* x_22; lean_object* x_23; lean_object* x_24; lean_object* x_25; lean_object* x_26; lean_object* x_27; lean_object* x_28; lean_object* x_29; lean_object* x_30; 
+x_3 = lean_ctor_get(x_1, 0);
+x_4 = lean_ctor_get(x_1, 1);
+x_5 = ((lean_object*)(lp_LDIRProofs_LDIR_instReprSIRInstruction_repr___redArg___closed__5));
+x_6 = ((lean_object*)(lp_LDIRProofs_LDIR_instReprSIRDocumentWithPayload_repr___redArg___closed__3));
+x_7 = lean_obj_once(&lp_LDIRProofs_LDIR_instReprSIRDocumentWithPayload_repr___redArg___closed__4, &lp_LDIRProofs_LDIR_instReprSIRDocumentWithPayload_repr___redArg___closed__4_once, _init_lp_LDIRProofs_LDIR_instReprSIRDocumentWithPayload_repr___redArg___closed__4);
+x_8 = lp_LDIRProofs_List_repr___at___00LDIR_instReprSIRDocumentWithPayload_repr_spec__0___redArg(x_3);
+lean_ctor_set_tag(x_1, 4);
+lean_ctor_set(x_1, 1, x_8);
+lean_ctor_set(x_1, 0, x_7);
+x_9 = 0;
+x_10 = lean_alloc_ctor(6, 1, 1);
+lean_ctor_set(x_10, 0, x_1);
+lean_ctor_set_uint8(x_10, sizeof(void*)*1, x_9);
+x_11 = lean_alloc_ctor(5, 2, 0);
+lean_ctor_set(x_11, 0, x_6);
+lean_ctor_set(x_11, 1, x_10);
+x_12 = ((lean_object*)(lp_LDIRProofs_LDIR_instReprSIRInstruction_repr___redArg___closed__9));
+x_13 = lean_alloc_ctor(5, 2, 0);
+lean_ctor_set(x_13, 0, x_11);
+lean_ctor_set(x_13, 1, x_12);
+x_14 = lean_box(1);
+x_15 = lean_alloc_ctor(5, 2, 0);
+lean_ctor_set(x_15, 0, x_13);
+lean_ctor_set(x_15, 1, x_14);
+x_16 = ((lean_object*)(lp_LDIRProofs_LDIR_instReprSIRDocumentWithPayload_repr___redArg___closed__6));
+x_17 = lean_alloc_ctor(5, 2, 0);
+lean_ctor_set(x_17, 0, x_15);
+lean_ctor_set(x_17, 1, x_16);
+x_18 = lean_alloc_ctor(5, 2, 0);
+lean_ctor_set(x_18, 0, x_17);
+lean_ctor_set(x_18, 1, x_5);
+x_19 = lean_obj_once(&lp_LDIRProofs_LDIR_instReprSIRDocumentWithPayload_repr___redArg___closed__7, &lp_LDIRProofs_LDIR_instReprSIRDocumentWithPayload_repr___redArg___closed__7_once, _init_lp_LDIRProofs_LDIR_instReprSIRDocumentWithPayload_repr___redArg___closed__7);
+x_20 = lp_LDIRProofs_LDIR_instReprPayloadTable_repr___redArg(x_4);
+x_21 = lean_alloc_ctor(4, 2, 0);
+lean_ctor_set(x_21, 0, x_19);
+lean_ctor_set(x_21, 1, x_20);
+x_22 = lean_alloc_ctor(6, 1, 1);
+lean_ctor_set(x_22, 0, x_21);
+lean_ctor_set_uint8(x_22, sizeof(void*)*1, x_9);
+x_23 = lean_alloc_ctor(5, 2, 0);
+lean_ctor_set(x_23, 0, x_18);
+lean_ctor_set(x_23, 1, x_22);
+x_24 = lean_obj_once(&lp_LDIRProofs_LDIR_instReprSIRInstruction_repr___redArg___closed__20, &lp_LDIRProofs_LDIR_instReprSIRInstruction_repr___redArg___closed__20_once, _init_lp_LDIRProofs_LDIR_instReprSIRInstruction_repr___redArg___closed__20);
+x_25 = ((lean_object*)(lp_LDIRProofs_LDIR_instReprSIRInstruction_repr___redArg___closed__21));
+x_26 = lean_alloc_ctor(5, 2, 0);
+lean_ctor_set(x_26, 0, x_25);
+lean_ctor_set(x_26, 1, x_23);
+x_27 = ((lean_object*)(lp_LDIRProofs_LDIR_instReprSIRInstruction_repr___redArg___closed__22));
+x_28 = lean_alloc_ctor(5, 2, 0);
+lean_ctor_set(x_28, 0, x_26);
+lean_ctor_set(x_28, 1, x_27);
+x_29 = lean_alloc_ctor(4, 2, 0);
+lean_ctor_set(x_29, 0, x_24);
+lean_ctor_set(x_29, 1, x_28);
+x_30 = lean_alloc_ctor(6, 1, 1);
+lean_ctor_set(x_30, 0, x_29);
+lean_ctor_set_uint8(x_30, sizeof(void*)*1, x_9);
+return x_30;
+}
+else
+{
+lean_object* x_31; lean_object* x_32; lean_object* x_33; lean_object* x_34; lean_object* x_35; lean_object* x_36; lean_object* x_37; uint8_t x_38; lean_object* x_39; lean_object* x_40; lean_object* x_41; lean_object* x_42; lean_object* x_43; lean_object* x_44; lean_object* x_45; lean_object* x_46; lean_object* x_47; lean_object* x_48; lean_object* x_49; lean_object* x_50; lean_object* x_51; lean_object* x_52; lean_object* x_53; lean_object* x_54; lean_object* x_55; lean_object* x_56; lean_object* x_57; lean_object* x_58; lean_object* x_59; 
+x_31 = lean_ctor_get(x_1, 0);
+x_32 = lean_ctor_get(x_1, 1);
+lean_inc(x_32);
+lean_inc(x_31);
+lean_dec(x_1);
+x_33 = ((lean_object*)(lp_LDIRProofs_LDIR_instReprSIRInstruction_repr___redArg___closed__5));
+x_34 = ((lean_object*)(lp_LDIRProofs_LDIR_instReprSIRDocumentWithPayload_repr___redArg___closed__3));
+x_35 = lean_obj_once(&lp_LDIRProofs_LDIR_instReprSIRDocumentWithPayload_repr___redArg___closed__4, &lp_LDIRProofs_LDIR_instReprSIRDocumentWithPayload_repr___redArg___closed__4_once, _init_lp_LDIRProofs_LDIR_instReprSIRDocumentWithPayload_repr___redArg___closed__4);
+x_36 = lp_LDIRProofs_List_repr___at___00LDIR_instReprSIRDocumentWithPayload_repr_spec__0___redArg(x_31);
+x_37 = lean_alloc_ctor(4, 2, 0);
+lean_ctor_set(x_37, 0, x_35);
+lean_ctor_set(x_37, 1, x_36);
+x_38 = 0;
+x_39 = lean_alloc_ctor(6, 1, 1);
+lean_ctor_set(x_39, 0, x_37);
+lean_ctor_set_uint8(x_39, sizeof(void*)*1, x_38);
+x_40 = lean_alloc_ctor(5, 2, 0);
+lean_ctor_set(x_40, 0, x_34);
+lean_ctor_set(x_40, 1, x_39);
+x_41 = ((lean_object*)(lp_LDIRProofs_LDIR_instReprSIRInstruction_repr___redArg___closed__9));
+x_42 = lean_alloc_ctor(5, 2, 0);
+lean_ctor_set(x_42, 0, x_40);
+lean_ctor_set(x_42, 1, x_41);
+x_43 = lean_box(1);
+x_44 = lean_alloc_ctor(5, 2, 0);
+lean_ctor_set(x_44, 0, x_42);
+lean_ctor_set(x_44, 1, x_43);
+x_45 = ((lean_object*)(lp_LDIRProofs_LDIR_instReprSIRDocumentWithPayload_repr___redArg___closed__6));
+x_46 = lean_alloc_ctor(5, 2, 0);
+lean_ctor_set(x_46, 0, x_44);
+lean_ctor_set(x_46, 1, x_45);
+x_47 = lean_alloc_ctor(5, 2, 0);
+lean_ctor_set(x_47, 0, x_46);
+lean_ctor_set(x_47, 1, x_33);
+x_48 = lean_obj_once(&lp_LDIRProofs_LDIR_instReprSIRDocumentWithPayload_repr___redArg___closed__7, &lp_LDIRProofs_LDIR_instReprSIRDocumentWithPayload_repr___redArg___closed__7_once, _init_lp_LDIRProofs_LDIR_instReprSIRDocumentWithPayload_repr___redArg___closed__7);
+x_49 = lp_LDIRProofs_LDIR_instReprPayloadTable_repr___redArg(x_32);
+x_50 = lean_alloc_ctor(4, 2, 0);
+lean_ctor_set(x_50, 0, x_48);
+lean_ctor_set(x_50, 1, x_49);
+x_51 = lean_alloc_ctor(6, 1, 1);
+lean_ctor_set(x_51, 0, x_50);
+lean_ctor_set_uint8(x_51, sizeof(void*)*1, x_38);
+x_52 = lean_alloc_ctor(5, 2, 0);
+lean_ctor_set(x_52, 0, x_47);
+lean_ctor_set(x_52, 1, x_51);
+x_53 = lean_obj_once(&lp_LDIRProofs_LDIR_instReprSIRInstruction_repr___redArg___closed__20, &lp_LDIRProofs_LDIR_instReprSIRInstruction_repr___redArg___closed__20_once, _init_lp_LDIRProofs_LDIR_instReprSIRInstruction_repr___redArg___closed__20);
+x_54 = ((lean_object*)(lp_LDIRProofs_LDIR_instReprSIRInstruction_repr___redArg___closed__21));
+x_55 = lean_alloc_ctor(5, 2, 0);
+lean_ctor_set(x_55, 0, x_54);
+lean_ctor_set(x_55, 1, x_52);
+x_56 = ((lean_object*)(lp_LDIRProofs_LDIR_instReprSIRInstruction_repr___redArg___closed__22));
+x_57 = lean_alloc_ctor(5, 2, 0);
+lean_ctor_set(x_57, 0, x_55);
+lean_ctor_set(x_57, 1, x_56);
+x_58 = lean_alloc_ctor(4, 2, 0);
+lean_ctor_set(x_58, 0, x_53);
+lean_ctor_set(x_58, 1, x_57);
+x_59 = lean_alloc_ctor(6, 1, 1);
+lean_ctor_set(x_59, 0, x_58);
+lean_ctor_set_uint8(x_59, sizeof(void*)*1, x_38);
+return x_59;
+}
+}
+}
+LEAN_EXPORT lean_object* lp_LDIRProofs_LDIR_instReprSIRDocumentWithPayload_repr(lean_object* x_1, lean_object* x_2) {
+_start:
+{
+lean_object* x_3; 
+x_3 = lp_LDIRProofs_LDIR_instReprSIRDocumentWithPayload_repr___redArg(x_1);
+return x_3;
+}
+}
+LEAN_EXPORT lean_object* lp_LDIRProofs_LDIR_instReprSIRDocumentWithPayload_repr___boxed(lean_object* x_1, lean_object* x_2) {
+_start:
+{
+lean_object* x_3; 
+x_3 = lp_LDIRProofs_LDIR_instReprSIRDocumentWithPayload_repr(x_1, x_2);
+lean_dec(x_2);
+return x_3;
+}
+}
+LEAN_EXPORT lean_object* lp_LDIRProofs_List_repr___at___00LDIR_instReprSIRDocumentWithPayload_repr_spec__0(lean_object* x_1, lean_object* x_2) {
+_start:
+{
+lean_object* x_3; 
+x_3 = lp_LDIRProofs_List_repr___at___00LDIR_instReprSIRDocumentWithPayload_repr_spec__0___redArg(x_1);
+return x_3;
+}
+}
+LEAN_EXPORT lean_object* lp_LDIRProofs_List_repr___at___00LDIR_instReprSIRDocumentWithPayload_repr_spec__0___boxed(lean_object* x_1, lean_object* x_2) {
+_start:
+{
+lean_object* x_3; 
+x_3 = lp_LDIRProofs_List_repr___at___00LDIR_instReprSIRDocumentWithPayload_repr_spec__0(x_1, x_2);
+lean_dec(x_2);
+return x_3;
+}
+}
+LEAN_EXPORT uint8_t lp_LDIRProofs_List_beq___at___00LDIR_instBEqSIRDocumentWithPayload_beq_spec__0(lean_object* x_1, lean_object* x_2) {
+_start:
+{
+if (lean_obj_tag(x_1) == 0)
+{
+if (lean_obj_tag(x_2) == 0)
+{
+uint8_t x_3; 
+x_3 = 1;
+return x_3;
+}
+else
+{
+uint8_t x_4; 
+x_4 = 0;
+return x_4;
+}
+}
+else
+{
+if (lean_obj_tag(x_2) == 0)
+{
+uint8_t x_5; 
+x_5 = 0;
+return x_5;
+}
+else
+{
+lean_object* x_6; lean_object* x_7; lean_object* x_8; lean_object* x_9; uint8_t x_10; 
+x_6 = lean_ctor_get(x_1, 0);
+x_7 = lean_ctor_get(x_1, 1);
+x_8 = lean_ctor_get(x_2, 0);
+x_9 = lean_ctor_get(x_2, 1);
+x_10 = lp_LDIRProofs_LDIR_instBEqSIRInstruction_beq(x_6, x_8);
+if (x_10 == 0)
+{
+return x_10;
+}
+else
+{
+x_1 = x_7;
+x_2 = x_9;
+goto _start;
+}
+}
+}
+}
+}
+LEAN_EXPORT lean_object* lp_LDIRProofs_List_beq___at___00LDIR_instBEqSIRDocumentWithPayload_beq_spec__0___boxed(lean_object* x_1, lean_object* x_2) {
+_start:
+{
+uint8_t x_3; lean_object* x_4; 
+x_3 = lp_LDIRProofs_List_beq___at___00LDIR_instBEqSIRDocumentWithPayload_beq_spec__0(x_1, x_2);
+lean_dec(x_2);
+lean_dec(x_1);
+x_4 = lean_box(x_3);
+return x_4;
+}
+}
+LEAN_EXPORT uint8_t lp_LDIRProofs_LDIR_instBEqSIRDocumentWithPayload_beq(lean_object* x_1, lean_object* x_2) {
+_start:
+{
+lean_object* x_3; lean_object* x_4; lean_object* x_5; lean_object* x_6; uint8_t x_7; 
+x_3 = lean_ctor_get(x_1, 0);
+x_4 = lean_ctor_get(x_1, 1);
+x_5 = lean_ctor_get(x_2, 0);
+x_6 = lean_ctor_get(x_2, 1);
+x_7 = lp_LDIRProofs_List_beq___at___00LDIR_instBEqSIRDocumentWithPayload_beq_spec__0(x_3, x_5);
+if (x_7 == 0)
+{
+return x_7;
+}
+else
+{
+uint8_t x_8; 
+x_8 = lean_string_dec_eq(x_4, x_6);
+return x_8;
+}
+}
+}
+LEAN_EXPORT lean_object* lp_LDIRProofs_LDIR_instBEqSIRDocumentWithPayload_beq___boxed(lean_object* x_1, lean_object* x_2) {
+_start:
+{
+uint8_t x_3; lean_object* x_4; 
+x_3 = lp_LDIRProofs_LDIR_instBEqSIRDocumentWithPayload_beq(x_1, x_2);
+lean_dec_ref(x_2);
+lean_dec_ref(x_1);
+x_4 = lean_box(x_3);
+return x_4;
+}
+}
+static lean_object* _init_lp_LDIRProofs_LDIR_GIR__COMMAND__ARGS(void) {
+_start:
+{
+lean_object* x_1; 
+x_1 = lean_unsigned_to_nat(8u);
+return x_1;
+}
+}
 LEAN_EXPORT lean_object* lp_LDIRProofs_LDIR_GIROpcode_ctorIdx(uint8_t x_1) {
 _start:
 {
@@ -2334,14 +3827,14 @@ x_53 = lean_nat_dec_le(x_52, x_2);
 if (x_53 == 0)
 {
 lean_object* x_54; 
-x_54 = lean_obj_once(&lp_LDIRProofs_LDIR_instReprBlockType_repr___closed__12, &lp_LDIRProofs_LDIR_instReprBlockType_repr___closed__12_once, _init_lp_LDIRProofs_LDIR_instReprBlockType_repr___closed__12);
+x_54 = lean_obj_once(&lp_LDIRProofs_LDIR_instReprBlockType_repr___closed__30, &lp_LDIRProofs_LDIR_instReprBlockType_repr___closed__30_once, _init_lp_LDIRProofs_LDIR_instReprBlockType_repr___closed__30);
 x_3 = x_54;
 goto block_9;
 }
 else
 {
 lean_object* x_55; 
-x_55 = lean_obj_once(&lp_LDIRProofs_LDIR_instReprBlockType_repr___closed__13, &lp_LDIRProofs_LDIR_instReprBlockType_repr___closed__13_once, _init_lp_LDIRProofs_LDIR_instReprBlockType_repr___closed__13);
+x_55 = lean_obj_once(&lp_LDIRProofs_LDIR_instReprBlockType_repr___closed__31, &lp_LDIRProofs_LDIR_instReprBlockType_repr___closed__31_once, _init_lp_LDIRProofs_LDIR_instReprBlockType_repr___closed__31);
 x_3 = x_55;
 goto block_9;
 }
@@ -2354,14 +3847,14 @@ x_57 = lean_nat_dec_le(x_56, x_2);
 if (x_57 == 0)
 {
 lean_object* x_58; 
-x_58 = lean_obj_once(&lp_LDIRProofs_LDIR_instReprBlockType_repr___closed__12, &lp_LDIRProofs_LDIR_instReprBlockType_repr___closed__12_once, _init_lp_LDIRProofs_LDIR_instReprBlockType_repr___closed__12);
+x_58 = lean_obj_once(&lp_LDIRProofs_LDIR_instReprBlockType_repr___closed__30, &lp_LDIRProofs_LDIR_instReprBlockType_repr___closed__30_once, _init_lp_LDIRProofs_LDIR_instReprBlockType_repr___closed__30);
 x_10 = x_58;
 goto block_16;
 }
 else
 {
 lean_object* x_59; 
-x_59 = lean_obj_once(&lp_LDIRProofs_LDIR_instReprBlockType_repr___closed__13, &lp_LDIRProofs_LDIR_instReprBlockType_repr___closed__13_once, _init_lp_LDIRProofs_LDIR_instReprBlockType_repr___closed__13);
+x_59 = lean_obj_once(&lp_LDIRProofs_LDIR_instReprBlockType_repr___closed__31, &lp_LDIRProofs_LDIR_instReprBlockType_repr___closed__31_once, _init_lp_LDIRProofs_LDIR_instReprBlockType_repr___closed__31);
 x_10 = x_59;
 goto block_16;
 }
@@ -2374,14 +3867,14 @@ x_61 = lean_nat_dec_le(x_60, x_2);
 if (x_61 == 0)
 {
 lean_object* x_62; 
-x_62 = lean_obj_once(&lp_LDIRProofs_LDIR_instReprBlockType_repr___closed__12, &lp_LDIRProofs_LDIR_instReprBlockType_repr___closed__12_once, _init_lp_LDIRProofs_LDIR_instReprBlockType_repr___closed__12);
+x_62 = lean_obj_once(&lp_LDIRProofs_LDIR_instReprBlockType_repr___closed__30, &lp_LDIRProofs_LDIR_instReprBlockType_repr___closed__30_once, _init_lp_LDIRProofs_LDIR_instReprBlockType_repr___closed__30);
 x_17 = x_62;
 goto block_23;
 }
 else
 {
 lean_object* x_63; 
-x_63 = lean_obj_once(&lp_LDIRProofs_LDIR_instReprBlockType_repr___closed__13, &lp_LDIRProofs_LDIR_instReprBlockType_repr___closed__13_once, _init_lp_LDIRProofs_LDIR_instReprBlockType_repr___closed__13);
+x_63 = lean_obj_once(&lp_LDIRProofs_LDIR_instReprBlockType_repr___closed__31, &lp_LDIRProofs_LDIR_instReprBlockType_repr___closed__31_once, _init_lp_LDIRProofs_LDIR_instReprBlockType_repr___closed__31);
 x_17 = x_63;
 goto block_23;
 }
@@ -2394,14 +3887,14 @@ x_65 = lean_nat_dec_le(x_64, x_2);
 if (x_65 == 0)
 {
 lean_object* x_66; 
-x_66 = lean_obj_once(&lp_LDIRProofs_LDIR_instReprBlockType_repr___closed__12, &lp_LDIRProofs_LDIR_instReprBlockType_repr___closed__12_once, _init_lp_LDIRProofs_LDIR_instReprBlockType_repr___closed__12);
+x_66 = lean_obj_once(&lp_LDIRProofs_LDIR_instReprBlockType_repr___closed__30, &lp_LDIRProofs_LDIR_instReprBlockType_repr___closed__30_once, _init_lp_LDIRProofs_LDIR_instReprBlockType_repr___closed__30);
 x_24 = x_66;
 goto block_30;
 }
 else
 {
 lean_object* x_67; 
-x_67 = lean_obj_once(&lp_LDIRProofs_LDIR_instReprBlockType_repr___closed__13, &lp_LDIRProofs_LDIR_instReprBlockType_repr___closed__13_once, _init_lp_LDIRProofs_LDIR_instReprBlockType_repr___closed__13);
+x_67 = lean_obj_once(&lp_LDIRProofs_LDIR_instReprBlockType_repr___closed__31, &lp_LDIRProofs_LDIR_instReprBlockType_repr___closed__31_once, _init_lp_LDIRProofs_LDIR_instReprBlockType_repr___closed__31);
 x_24 = x_67;
 goto block_30;
 }
@@ -2414,14 +3907,14 @@ x_69 = lean_nat_dec_le(x_68, x_2);
 if (x_69 == 0)
 {
 lean_object* x_70; 
-x_70 = lean_obj_once(&lp_LDIRProofs_LDIR_instReprBlockType_repr___closed__12, &lp_LDIRProofs_LDIR_instReprBlockType_repr___closed__12_once, _init_lp_LDIRProofs_LDIR_instReprBlockType_repr___closed__12);
+x_70 = lean_obj_once(&lp_LDIRProofs_LDIR_instReprBlockType_repr___closed__30, &lp_LDIRProofs_LDIR_instReprBlockType_repr___closed__30_once, _init_lp_LDIRProofs_LDIR_instReprBlockType_repr___closed__30);
 x_31 = x_70;
 goto block_37;
 }
 else
 {
 lean_object* x_71; 
-x_71 = lean_obj_once(&lp_LDIRProofs_LDIR_instReprBlockType_repr___closed__13, &lp_LDIRProofs_LDIR_instReprBlockType_repr___closed__13_once, _init_lp_LDIRProofs_LDIR_instReprBlockType_repr___closed__13);
+x_71 = lean_obj_once(&lp_LDIRProofs_LDIR_instReprBlockType_repr___closed__31, &lp_LDIRProofs_LDIR_instReprBlockType_repr___closed__31_once, _init_lp_LDIRProofs_LDIR_instReprBlockType_repr___closed__31);
 x_31 = x_71;
 goto block_37;
 }
@@ -2434,14 +3927,14 @@ x_73 = lean_nat_dec_le(x_72, x_2);
 if (x_73 == 0)
 {
 lean_object* x_74; 
-x_74 = lean_obj_once(&lp_LDIRProofs_LDIR_instReprBlockType_repr___closed__12, &lp_LDIRProofs_LDIR_instReprBlockType_repr___closed__12_once, _init_lp_LDIRProofs_LDIR_instReprBlockType_repr___closed__12);
+x_74 = lean_obj_once(&lp_LDIRProofs_LDIR_instReprBlockType_repr___closed__30, &lp_LDIRProofs_LDIR_instReprBlockType_repr___closed__30_once, _init_lp_LDIRProofs_LDIR_instReprBlockType_repr___closed__30);
 x_38 = x_74;
 goto block_44;
 }
 else
 {
 lean_object* x_75; 
-x_75 = lean_obj_once(&lp_LDIRProofs_LDIR_instReprBlockType_repr___closed__13, &lp_LDIRProofs_LDIR_instReprBlockType_repr___closed__13_once, _init_lp_LDIRProofs_LDIR_instReprBlockType_repr___closed__13);
+x_75 = lean_obj_once(&lp_LDIRProofs_LDIR_instReprBlockType_repr___closed__31, &lp_LDIRProofs_LDIR_instReprBlockType_repr___closed__31_once, _init_lp_LDIRProofs_LDIR_instReprBlockType_repr___closed__31);
 x_38 = x_75;
 goto block_44;
 }
@@ -2454,14 +3947,14 @@ x_77 = lean_nat_dec_le(x_76, x_2);
 if (x_77 == 0)
 {
 lean_object* x_78; 
-x_78 = lean_obj_once(&lp_LDIRProofs_LDIR_instReprBlockType_repr___closed__12, &lp_LDIRProofs_LDIR_instReprBlockType_repr___closed__12_once, _init_lp_LDIRProofs_LDIR_instReprBlockType_repr___closed__12);
+x_78 = lean_obj_once(&lp_LDIRProofs_LDIR_instReprBlockType_repr___closed__30, &lp_LDIRProofs_LDIR_instReprBlockType_repr___closed__30_once, _init_lp_LDIRProofs_LDIR_instReprBlockType_repr___closed__30);
 x_45 = x_78;
 goto block_51;
 }
 else
 {
 lean_object* x_79; 
-x_79 = lean_obj_once(&lp_LDIRProofs_LDIR_instReprBlockType_repr___closed__13, &lp_LDIRProofs_LDIR_instReprBlockType_repr___closed__13_once, _init_lp_LDIRProofs_LDIR_instReprBlockType_repr___closed__13);
+x_79 = lean_obj_once(&lp_LDIRProofs_LDIR_instReprBlockType_repr___closed__31, &lp_LDIRProofs_LDIR_instReprBlockType_repr___closed__31_once, _init_lp_LDIRProofs_LDIR_instReprBlockType_repr___closed__31);
 x_45 = x_79;
 goto block_51;
 }
@@ -2713,7 +4206,7 @@ x_6 = lean_box(x_5);
 return x_6;
 }
 }
-static lean_object* _init_lp_LDIRProofs_LDIR_instReprGIRCommand_repr___redArg___closed__4(void) {
+static lean_object* _init_lp_LDIRProofs_LDIR_GIRCommand_zeroed___lam__0___closed__0(void) {
 _start:
 {
 lean_object* x_1; lean_object* x_2; 
@@ -2722,183 +4215,120 @@ x_2 = lean_nat_to_int(x_1);
 return x_2;
 }
 }
-LEAN_EXPORT lean_object* lp_LDIRProofs_LDIR_instReprGIRCommand_repr___redArg(lean_object* x_1) {
+LEAN_EXPORT lean_object* lp_LDIRProofs_LDIR_GIRCommand_zeroed___lam__0(lean_object* x_1) {
 _start:
 {
-uint8_t x_2; lean_object* x_3; lean_object* x_4; lean_object* x_5; lean_object* x_6; lean_object* x_7; lean_object* x_8; lean_object* x_9; lean_object* x_10; uint8_t x_11; lean_object* x_12; lean_object* x_13; lean_object* x_14; lean_object* x_15; lean_object* x_16; lean_object* x_17; lean_object* x_18; lean_object* x_19; lean_object* x_20; lean_object* x_21; lean_object* x_43; uint8_t x_44; 
-x_2 = lean_ctor_get_uint8(x_1, sizeof(void*)*2);
-x_3 = lean_ctor_get(x_1, 0);
+lean_object* x_2; 
+x_2 = lean_obj_once(&lp_LDIRProofs_LDIR_GIRCommand_zeroed___lam__0___closed__0, &lp_LDIRProofs_LDIR_GIRCommand_zeroed___lam__0___closed__0_once, _init_lp_LDIRProofs_LDIR_GIRCommand_zeroed___lam__0___closed__0);
+return x_2;
+}
+}
+LEAN_EXPORT lean_object* lp_LDIRProofs_LDIR_GIRCommand_zeroed___lam__0___boxed(lean_object* x_1) {
+_start:
+{
+lean_object* x_2; 
+x_2 = lp_LDIRProofs_LDIR_GIRCommand_zeroed___lam__0(x_1);
+lean_dec(x_1);
+return x_2;
+}
+}
+LEAN_EXPORT lean_object* lp_LDIRProofs_LDIR_GIRCommand_zeroed(uint8_t x_1) {
+_start:
+{
+lean_object* x_2; lean_object* x_3; 
+x_2 = ((lean_object*)(lp_LDIRProofs_LDIR_GIRCommand_zeroed___closed__0));
+x_3 = lean_alloc_ctor(0, 1, 1);
+lean_ctor_set(x_3, 0, x_2);
+lean_ctor_set_uint8(x_3, sizeof(void*)*1, x_1);
+return x_3;
+}
+}
+LEAN_EXPORT lean_object* lp_LDIRProofs_LDIR_GIRCommand_zeroed___boxed(lean_object* x_1) {
+_start:
+{
+uint8_t x_2; lean_object* x_3; 
+x_2 = lean_unbox(x_1);
+x_3 = lp_LDIRProofs_LDIR_GIRCommand_zeroed(x_2);
+return x_3;
+}
+}
+LEAN_EXPORT uint8_t lp_LDIRProofs_LDIR_instBEqGIRCommand___lam__0(lean_object* x_1, lean_object* x_2, lean_object* x_3) {
+_start:
+{
+lean_object* x_4; lean_object* x_5; uint8_t x_6; 
 lean_inc(x_3);
-x_4 = lean_ctor_get(x_1, 1);
+x_4 = lean_apply_1(x_1, x_3);
+x_5 = lean_apply_1(x_2, x_3);
+x_6 = lean_int_dec_eq(x_4, x_5);
+lean_dec(x_5);
+lean_dec(x_4);
+return x_6;
+}
+}
+LEAN_EXPORT lean_object* lp_LDIRProofs_LDIR_instBEqGIRCommand___lam__0___boxed(lean_object* x_1, lean_object* x_2, lean_object* x_3) {
+_start:
+{
+uint8_t x_4; lean_object* x_5; 
+x_4 = lp_LDIRProofs_LDIR_instBEqGIRCommand___lam__0(x_1, x_2, x_3);
+x_5 = lean_box(x_4);
+return x_5;
+}
+}
+LEAN_EXPORT uint8_t lp_LDIRProofs_LDIR_instBEqGIRCommand___lam__1(lean_object* x_1, lean_object* x_2) {
+_start:
+{
+uint8_t x_3; lean_object* x_4; uint8_t x_5; lean_object* x_6; uint8_t x_7; 
+x_3 = lean_ctor_get_uint8(x_1, sizeof(void*)*1);
+x_4 = lean_ctor_get(x_1, 0);
 lean_inc_ref(x_4);
 lean_dec_ref(x_1);
-x_5 = ((lean_object*)(lp_LDIRProofs_LDIR_instReprSIRInstruction_repr___redArg___closed__5));
-x_6 = ((lean_object*)(lp_LDIRProofs_LDIR_instReprSIRInstruction_repr___redArg___closed__6));
-x_7 = lean_obj_once(&lp_LDIRProofs_LDIR_instReprSIRInstruction_repr___redArg___closed__7, &lp_LDIRProofs_LDIR_instReprSIRInstruction_repr___redArg___closed__7_once, _init_lp_LDIRProofs_LDIR_instReprSIRInstruction_repr___redArg___closed__7);
-x_8 = lean_unsigned_to_nat(0u);
-x_9 = lp_LDIRProofs_LDIR_instReprGIROpcode_repr(x_2, x_8);
-x_10 = lean_alloc_ctor(4, 2, 0);
-lean_ctor_set(x_10, 0, x_7);
-lean_ctor_set(x_10, 1, x_9);
-x_11 = 0;
-x_12 = lean_alloc_ctor(6, 1, 1);
-lean_ctor_set(x_12, 0, x_10);
-lean_ctor_set_uint8(x_12, sizeof(void*)*1, x_11);
-x_13 = lean_alloc_ctor(5, 2, 0);
-lean_ctor_set(x_13, 0, x_6);
-lean_ctor_set(x_13, 1, x_12);
-x_14 = ((lean_object*)(lp_LDIRProofs_LDIR_instReprSIRInstruction_repr___redArg___closed__9));
-x_15 = lean_alloc_ctor(5, 2, 0);
-lean_ctor_set(x_15, 0, x_13);
-lean_ctor_set(x_15, 1, x_14);
-x_16 = lean_box(1);
-x_17 = lean_alloc_ctor(5, 2, 0);
-lean_ctor_set(x_17, 0, x_15);
-lean_ctor_set(x_17, 1, x_16);
-x_18 = ((lean_object*)(lp_LDIRProofs_LDIR_instReprGIRCommand_repr___redArg___closed__1));
-x_19 = lean_alloc_ctor(5, 2, 0);
-lean_ctor_set(x_19, 0, x_17);
-lean_ctor_set(x_19, 1, x_18);
-x_20 = lean_alloc_ctor(5, 2, 0);
-lean_ctor_set(x_20, 0, x_19);
-lean_ctor_set(x_20, 1, x_5);
-x_43 = lean_obj_once(&lp_LDIRProofs_LDIR_instReprGIRCommand_repr___redArg___closed__4, &lp_LDIRProofs_LDIR_instReprGIRCommand_repr___redArg___closed__4_once, _init_lp_LDIRProofs_LDIR_instReprGIRCommand_repr___redArg___closed__4);
-x_44 = lean_int_dec_lt(x_3, x_43);
-if (x_44 == 0)
+x_5 = lean_ctor_get_uint8(x_2, sizeof(void*)*1);
+x_6 = lean_ctor_get(x_2, 0);
+lean_inc_ref(x_6);
+lean_dec_ref(x_2);
+x_7 = lp_LDIRProofs_LDIR_instBEqGIROpcode_beq(x_3, x_5);
+if (x_7 == 0)
 {
-lean_object* x_45; lean_object* x_46; 
-x_45 = l_Int_repr(x_3);
-lean_dec(x_3);
-x_46 = lean_alloc_ctor(3, 1, 0);
-lean_ctor_set(x_46, 0, x_45);
-x_21 = x_46;
-goto block_42;
+lean_dec_ref(x_6);
+lean_dec_ref(x_4);
+return x_7;
 }
 else
 {
-lean_object* x_47; lean_object* x_48; lean_object* x_49; 
-x_47 = l_Int_repr(x_3);
-lean_dec(x_3);
-x_48 = lean_alloc_ctor(3, 1, 0);
-lean_ctor_set(x_48, 0, x_47);
-x_49 = l_Repr_addAppParen(x_48, x_8);
-x_21 = x_49;
-goto block_42;
-}
-block_42:
-{
-lean_object* x_22; lean_object* x_23; lean_object* x_24; lean_object* x_25; lean_object* x_26; lean_object* x_27; lean_object* x_28; lean_object* x_29; lean_object* x_30; lean_object* x_31; lean_object* x_32; lean_object* x_33; lean_object* x_34; lean_object* x_35; lean_object* x_36; lean_object* x_37; lean_object* x_38; lean_object* x_39; lean_object* x_40; lean_object* x_41; 
-x_22 = lean_alloc_ctor(4, 2, 0);
-lean_ctor_set(x_22, 0, x_7);
-lean_ctor_set(x_22, 1, x_21);
-x_23 = lean_alloc_ctor(6, 1, 1);
-lean_ctor_set(x_23, 0, x_22);
-lean_ctor_set_uint8(x_23, sizeof(void*)*1, x_11);
-x_24 = lean_alloc_ctor(5, 2, 0);
-lean_ctor_set(x_24, 0, x_20);
-lean_ctor_set(x_24, 1, x_23);
-x_25 = lean_alloc_ctor(5, 2, 0);
-lean_ctor_set(x_25, 0, x_24);
-lean_ctor_set(x_25, 1, x_14);
-x_26 = lean_alloc_ctor(5, 2, 0);
-lean_ctor_set(x_26, 0, x_25);
-lean_ctor_set(x_26, 1, x_16);
-x_27 = ((lean_object*)(lp_LDIRProofs_LDIR_instReprGIRCommand_repr___redArg___closed__3));
-x_28 = lean_alloc_ctor(5, 2, 0);
-lean_ctor_set(x_28, 0, x_26);
-lean_ctor_set(x_28, 1, x_27);
-x_29 = lean_alloc_ctor(5, 2, 0);
-lean_ctor_set(x_29, 0, x_28);
-lean_ctor_set(x_29, 1, x_5);
-x_30 = l_String_quote(x_4);
-x_31 = lean_alloc_ctor(3, 1, 0);
-lean_ctor_set(x_31, 0, x_30);
-x_32 = lean_alloc_ctor(4, 2, 0);
-lean_ctor_set(x_32, 0, x_7);
-lean_ctor_set(x_32, 1, x_31);
-x_33 = lean_alloc_ctor(6, 1, 1);
-lean_ctor_set(x_33, 0, x_32);
-lean_ctor_set_uint8(x_33, sizeof(void*)*1, x_11);
-x_34 = lean_alloc_ctor(5, 2, 0);
-lean_ctor_set(x_34, 0, x_29);
-lean_ctor_set(x_34, 1, x_33);
-x_35 = lean_obj_once(&lp_LDIRProofs_LDIR_instReprSIRInstruction_repr___redArg___closed__20, &lp_LDIRProofs_LDIR_instReprSIRInstruction_repr___redArg___closed__20_once, _init_lp_LDIRProofs_LDIR_instReprSIRInstruction_repr___redArg___closed__20);
-x_36 = ((lean_object*)(lp_LDIRProofs_LDIR_instReprSIRInstruction_repr___redArg___closed__21));
-x_37 = lean_alloc_ctor(5, 2, 0);
-lean_ctor_set(x_37, 0, x_36);
-lean_ctor_set(x_37, 1, x_34);
-x_38 = ((lean_object*)(lp_LDIRProofs_LDIR_instReprSIRInstruction_repr___redArg___closed__22));
-x_39 = lean_alloc_ctor(5, 2, 0);
-lean_ctor_set(x_39, 0, x_37);
-lean_ctor_set(x_39, 1, x_38);
-x_40 = lean_alloc_ctor(4, 2, 0);
-lean_ctor_set(x_40, 0, x_35);
-lean_ctor_set(x_40, 1, x_39);
-x_41 = lean_alloc_ctor(6, 1, 1);
-lean_ctor_set(x_41, 0, x_40);
-lean_ctor_set_uint8(x_41, sizeof(void*)*1, x_11);
-return x_41;
-}
-}
-}
-LEAN_EXPORT lean_object* lp_LDIRProofs_LDIR_instReprGIRCommand_repr(lean_object* x_1, lean_object* x_2) {
-_start:
-{
-lean_object* x_3; 
-x_3 = lp_LDIRProofs_LDIR_instReprGIRCommand_repr___redArg(x_1);
-return x_3;
-}
-}
-LEAN_EXPORT lean_object* lp_LDIRProofs_LDIR_instReprGIRCommand_repr___boxed(lean_object* x_1, lean_object* x_2) {
-_start:
-{
-lean_object* x_3; 
-x_3 = lp_LDIRProofs_LDIR_instReprGIRCommand_repr(x_1, x_2);
-lean_dec(x_2);
-return x_3;
-}
-}
-LEAN_EXPORT uint8_t lp_LDIRProofs_LDIR_instBEqGIRCommand_beq(lean_object* x_1, lean_object* x_2) {
-_start:
-{
-uint8_t x_3; lean_object* x_4; lean_object* x_5; uint8_t x_6; lean_object* x_7; lean_object* x_8; uint8_t x_9; 
-x_3 = lean_ctor_get_uint8(x_1, sizeof(void*)*2);
-x_4 = lean_ctor_get(x_1, 0);
-x_5 = lean_ctor_get(x_1, 1);
-x_6 = lean_ctor_get_uint8(x_2, sizeof(void*)*2);
-x_7 = lean_ctor_get(x_2, 0);
-x_8 = lean_ctor_get(x_2, 1);
-x_9 = lp_LDIRProofs_LDIR_instBEqGIROpcode_beq(x_3, x_6);
-if (x_9 == 0)
-{
-return x_9;
-}
-else
-{
-uint8_t x_10; 
-x_10 = lean_int_dec_eq(x_4, x_7);
-if (x_10 == 0)
-{
+lean_object* x_8; lean_object* x_9; uint8_t x_10; 
+x_8 = lean_alloc_closure((void*)(lp_LDIRProofs_LDIR_instBEqGIRCommand___lam__0___boxed), 3, 2);
+lean_closure_set(x_8, 0, x_4);
+lean_closure_set(x_8, 1, x_6);
+x_9 = lean_unsigned_to_nat(8u);
+x_10 = l_Nat_decidableForallFin___redArg(x_9, x_8);
 return x_10;
 }
-else
-{
-uint8_t x_11; 
-x_11 = lean_string_dec_eq(x_5, x_8);
-return x_11;
 }
 }
-}
-}
-LEAN_EXPORT lean_object* lp_LDIRProofs_LDIR_instBEqGIRCommand_beq___boxed(lean_object* x_1, lean_object* x_2) {
+LEAN_EXPORT lean_object* lp_LDIRProofs_LDIR_instBEqGIRCommand___lam__1___boxed(lean_object* x_1, lean_object* x_2) {
 _start:
 {
 uint8_t x_3; lean_object* x_4; 
-x_3 = lp_LDIRProofs_LDIR_instBEqGIRCommand_beq(x_1, x_2);
-lean_dec_ref(x_2);
-lean_dec_ref(x_1);
+x_3 = lp_LDIRProofs_LDIR_instBEqGIRCommand___lam__1(x_1, x_2);
 x_4 = lean_box(x_3);
 return x_4;
+}
+}
+static lean_object* _init_lp_LDIRProofs_LDIR_instInhabitedGIRCommand___closed__0(void) {
+_start:
+{
+uint8_t x_1; lean_object* x_2; 
+x_1 = 0;
+x_2 = lp_LDIRProofs_LDIR_GIRCommand_zeroed(x_1);
+return x_2;
+}
+}
+static lean_object* _init_lp_LDIRProofs_LDIR_instInhabitedGIRCommand(void) {
+_start:
+{
+lean_object* x_1; 
+x_1 = lean_obj_once(&lp_LDIRProofs_LDIR_instInhabitedGIRCommand___closed__0, &lp_LDIRProofs_LDIR_instInhabitedGIRCommand___closed__0_once, _init_lp_LDIRProofs_LDIR_instInhabitedGIRCommand___closed__0);
+return x_1;
 }
 }
 LEAN_EXPORT lean_object* lp_LDIRProofs_List_mapTR_loop___at___00LDIR_entityUnique_spec__0(lean_object* x_1, lean_object* x_2) {
@@ -3149,26 +4579,214 @@ x_3 = lean_box(x_2);
 return x_3;
 }
 }
-LEAN_EXPORT uint8_t lp_LDIRProofs_LDIR_wellFormedSIR(lean_object* x_1) {
+LEAN_EXPORT uint8_t lp_LDIRProofs_LDIR_isAcyclicAux___lam__0(lean_object* x_1, lean_object* x_2) {
 _start:
 {
-uint8_t x_2; uint8_t x_5; 
-lean_inc(x_1);
-x_5 = lp_LDIRProofs_LDIR_entityUnique(x_1);
-if (x_5 == 0)
+lean_object* x_3; uint8_t x_4; 
+x_3 = lean_ctor_get(x_2, 1);
+x_4 = lean_nat_dec_eq(x_3, x_1);
+return x_4;
+}
+}
+LEAN_EXPORT lean_object* lp_LDIRProofs_LDIR_isAcyclicAux___lam__0___boxed(lean_object* x_1, lean_object* x_2) {
+_start:
 {
-x_2 = x_5;
-goto block_4;
+uint8_t x_3; lean_object* x_4; 
+x_3 = lp_LDIRProofs_LDIR_isAcyclicAux___lam__0(x_1, x_2);
+lean_dec_ref(x_2);
+lean_dec(x_1);
+x_4 = lean_box(x_3);
+return x_4;
+}
+}
+LEAN_EXPORT uint8_t lp_LDIRProofs_LDIR_isAcyclicAux(lean_object* x_1, lean_object* x_2, lean_object* x_3) {
+_start:
+{
+lean_object* x_4; uint8_t x_5; 
+x_4 = lean_unsigned_to_nat(0u);
+x_5 = lean_nat_dec_eq(x_3, x_4);
+if (x_5 == 1)
+{
+uint8_t x_6; 
+lean_dec(x_3);
+lean_dec(x_2);
+lean_dec(x_1);
+x_6 = 0;
+return x_6;
 }
 else
 {
-uint8_t x_6; 
+lean_object* x_7; lean_object* x_8; 
+x_7 = lean_alloc_closure((void*)(lp_LDIRProofs_LDIR_isAcyclicAux___lam__0___boxed), 2, 1);
+lean_closure_set(x_7, 0, x_2);
 lean_inc(x_1);
-x_6 = lp_LDIRProofs_LDIR_parentExists(x_1);
-x_2 = x_6;
-goto block_4;
+x_8 = l_List_find_x3f___redArg(x_7, x_1);
+if (lean_obj_tag(x_8) == 0)
+{
+uint8_t x_9; 
+lean_dec(x_3);
+lean_dec(x_1);
+x_9 = 1;
+return x_9;
 }
-block_4:
+else
+{
+lean_object* x_10; lean_object* x_11; lean_object* x_12; uint8_t x_13; 
+x_10 = lean_ctor_get(x_8, 0);
+lean_inc(x_10);
+lean_dec_ref(x_8);
+x_11 = lean_ctor_get(x_10, 2);
+lean_inc(x_11);
+lean_dec(x_10);
+x_12 = lean_unsigned_to_nat(4294967295u);
+x_13 = lean_nat_dec_eq(x_11, x_12);
+if (x_13 == 0)
+{
+lean_object* x_14; lean_object* x_15; 
+x_14 = lean_unsigned_to_nat(1u);
+x_15 = lean_nat_sub(x_3, x_14);
+lean_dec(x_3);
+x_2 = x_11;
+x_3 = x_15;
+goto _start;
+}
+else
+{
+lean_dec(x_11);
+lean_dec(x_3);
+lean_dec(x_1);
+return x_13;
+}
+}
+}
+}
+}
+LEAN_EXPORT lean_object* lp_LDIRProofs_LDIR_isAcyclicAux___boxed(lean_object* x_1, lean_object* x_2, lean_object* x_3) {
+_start:
+{
+uint8_t x_4; lean_object* x_5; 
+x_4 = lp_LDIRProofs_LDIR_isAcyclicAux(x_1, x_2, x_3);
+x_5 = lean_box(x_4);
+return x_5;
+}
+}
+LEAN_EXPORT uint8_t lp_LDIRProofs_LDIR_isAcyclic___lam__0(lean_object* x_1, lean_object* x_2) {
+_start:
+{
+lean_object* x_3; lean_object* x_4; uint8_t x_5; 
+x_3 = lean_ctor_get(x_2, 1);
+lean_inc(x_3);
+lean_dec_ref(x_2);
+x_4 = l_List_lengthTR___redArg(x_1);
+x_5 = lp_LDIRProofs_LDIR_isAcyclicAux(x_1, x_3, x_4);
+return x_5;
+}
+}
+LEAN_EXPORT lean_object* lp_LDIRProofs_LDIR_isAcyclic___lam__0___boxed(lean_object* x_1, lean_object* x_2) {
+_start:
+{
+uint8_t x_3; lean_object* x_4; 
+x_3 = lp_LDIRProofs_LDIR_isAcyclic___lam__0(x_1, x_2);
+x_4 = lean_box(x_3);
+return x_4;
+}
+}
+LEAN_EXPORT uint8_t lp_LDIRProofs_LDIR_isAcyclic(lean_object* x_1) {
+_start:
+{
+lean_object* x_2; uint8_t x_3; 
+lean_inc(x_1);
+x_2 = lean_alloc_closure((void*)(lp_LDIRProofs_LDIR_isAcyclic___lam__0___boxed), 2, 1);
+lean_closure_set(x_2, 0, x_1);
+x_3 = l_List_all___redArg(x_1, x_2);
+return x_3;
+}
+}
+LEAN_EXPORT lean_object* lp_LDIRProofs_LDIR_isAcyclic___boxed(lean_object* x_1) {
+_start:
+{
+uint8_t x_2; lean_object* x_3; 
+x_2 = lp_LDIRProofs_LDIR_isAcyclic(x_1);
+x_3 = lean_box(x_2);
+return x_3;
+}
+}
+LEAN_EXPORT uint8_t lp_LDIRProofs_LDIR_payloadValid___lam__0(lean_object* x_1, lean_object* x_2) {
+_start:
+{
+lean_object* x_3; 
+x_3 = lean_ctor_get(x_2, 0);
+if (lean_obj_tag(x_3) == 2)
+{
+uint8_t x_4; 
+x_4 = 1;
+return x_4;
+}
+else
+{
+lean_object* x_5; lean_object* x_6; uint8_t x_7; 
+x_5 = lean_ctor_get(x_2, 3);
+x_6 = lean_string_length(x_1);
+x_7 = lean_nat_dec_lt(x_5, x_6);
+return x_7;
+}
+}
+}
+LEAN_EXPORT lean_object* lp_LDIRProofs_LDIR_payloadValid___lam__0___boxed(lean_object* x_1, lean_object* x_2) {
+_start:
+{
+uint8_t x_3; lean_object* x_4; 
+x_3 = lp_LDIRProofs_LDIR_payloadValid___lam__0(x_1, x_2);
+lean_dec_ref(x_2);
+lean_dec_ref(x_1);
+x_4 = lean_box(x_3);
+return x_4;
+}
+}
+LEAN_EXPORT uint8_t lp_LDIRProofs_LDIR_payloadValid(lean_object* x_1) {
+_start:
+{
+lean_object* x_2; lean_object* x_3; lean_object* x_4; uint8_t x_5; 
+x_2 = lean_ctor_get(x_1, 0);
+lean_inc(x_2);
+x_3 = lean_ctor_get(x_1, 1);
+lean_inc_ref(x_3);
+lean_dec_ref(x_1);
+x_4 = lean_alloc_closure((void*)(lp_LDIRProofs_LDIR_payloadValid___lam__0___boxed), 2, 1);
+lean_closure_set(x_4, 0, x_3);
+x_5 = l_List_all___redArg(x_2, x_4);
+return x_5;
+}
+}
+LEAN_EXPORT lean_object* lp_LDIRProofs_LDIR_payloadValid___boxed(lean_object* x_1) {
+_start:
+{
+uint8_t x_2; lean_object* x_3; 
+x_2 = lp_LDIRProofs_LDIR_payloadValid(x_1);
+x_3 = lean_box(x_2);
+return x_3;
+}
+}
+LEAN_EXPORT uint8_t lp_LDIRProofs_LDIR_wellFormedSIR(lean_object* x_1) {
+_start:
+{
+uint8_t x_2; uint8_t x_6; 
+lean_inc(x_1);
+x_6 = lp_LDIRProofs_LDIR_entityUnique(x_1);
+if (x_6 == 0)
+{
+x_2 = x_6;
+goto block_5;
+}
+else
+{
+uint8_t x_7; 
+lean_inc(x_1);
+x_7 = lp_LDIRProofs_LDIR_parentExists(x_1);
+x_2 = x_7;
+goto block_5;
+}
+block_5:
 {
 if (x_2 == 0)
 {
@@ -3178,8 +4796,19 @@ return x_2;
 else
 {
 uint8_t x_3; 
-x_3 = lp_LDIRProofs_LDIR_hasSingleRoot(x_1);
+lean_inc(x_1);
+x_3 = lp_LDIRProofs_LDIR_isAcyclic(x_1);
+if (x_3 == 0)
+{
+lean_dec(x_1);
 return x_3;
+}
+else
+{
+uint8_t x_4; 
+x_4 = lp_LDIRProofs_LDIR_hasSingleRoot(x_1);
+return x_4;
+}
 }
 }
 }
@@ -3189,6 +4818,35 @@ _start:
 {
 uint8_t x_2; lean_object* x_3; 
 x_2 = lp_LDIRProofs_LDIR_wellFormedSIR(x_1);
+x_3 = lean_box(x_2);
+return x_3;
+}
+}
+LEAN_EXPORT uint8_t lp_LDIRProofs_LDIR_wellFormedSIRWithPayload(lean_object* x_1) {
+_start:
+{
+lean_object* x_2; uint8_t x_3; 
+x_2 = lean_ctor_get(x_1, 0);
+lean_inc(x_2);
+x_3 = lp_LDIRProofs_LDIR_wellFormedSIR(x_2);
+if (x_3 == 0)
+{
+lean_dec_ref(x_1);
+return x_3;
+}
+else
+{
+uint8_t x_4; 
+x_4 = lp_LDIRProofs_LDIR_payloadValid(x_1);
+return x_4;
+}
+}
+}
+LEAN_EXPORT lean_object* lp_LDIRProofs_LDIR_wellFormedSIRWithPayload___boxed(lean_object* x_1) {
+_start:
+{
+uint8_t x_2; lean_object* x_3; 
+x_2 = lp_LDIRProofs_LDIR_wellFormedSIRWithPayload(x_1);
 x_3 = lean_box(x_2);
 return x_3;
 }
@@ -3208,7 +4866,7 @@ else
 {
 lean_object* x_5; uint8_t x_6; 
 x_5 = lean_ctor_get(x_1, 0);
-x_6 = lean_ctor_get_uint8(x_5, sizeof(void*)*2);
+x_6 = lean_ctor_get_uint8(x_5, sizeof(void*)*1);
 switch (x_6) {
 case 4:
 {
@@ -3472,6 +5130,208 @@ x_7 = lp_LDIRProofs___private_LDIRProofs_proof__ir__wellformedness_0__LDIR_stack
 return x_7;
 }
 }
+LEAN_EXPORT lean_object* lp_LDIRProofs___private_LDIRProofs_proof__ir__wellformedness_0__List_any_match__1_splitter___redArg(lean_object* x_1, lean_object* x_2, lean_object* x_3, lean_object* x_4) {
+_start:
+{
+if (lean_obj_tag(x_1) == 0)
+{
+lean_object* x_5; 
+lean_dec(x_4);
+x_5 = lean_apply_1(x_3, x_2);
+return x_5;
+}
+else
+{
+lean_object* x_6; lean_object* x_7; lean_object* x_8; 
+lean_dec(x_3);
+x_6 = lean_ctor_get(x_1, 0);
+lean_inc(x_6);
+x_7 = lean_ctor_get(x_1, 1);
+lean_inc(x_7);
+lean_dec_ref(x_1);
+x_8 = lean_apply_3(x_4, x_6, x_7, x_2);
+return x_8;
+}
+}
+}
+LEAN_EXPORT lean_object* lp_LDIRProofs___private_LDIRProofs_proof__ir__wellformedness_0__List_any_match__1_splitter(lean_object* x_1, lean_object* x_2, lean_object* x_3, lean_object* x_4, lean_object* x_5, lean_object* x_6) {
+_start:
+{
+if (lean_obj_tag(x_3) == 0)
+{
+lean_object* x_7; 
+lean_dec(x_6);
+x_7 = lean_apply_1(x_5, x_4);
+return x_7;
+}
+else
+{
+lean_object* x_8; lean_object* x_9; lean_object* x_10; 
+lean_dec(x_5);
+x_8 = lean_ctor_get(x_3, 0);
+lean_inc(x_8);
+x_9 = lean_ctor_get(x_3, 1);
+lean_inc(x_9);
+lean_dec_ref(x_3);
+x_10 = lean_apply_3(x_6, x_8, x_9, x_4);
+return x_10;
+}
+}
+}
+LEAN_EXPORT lean_object* lp_LDIRProofs___private_LDIRProofs_proof__ir__wellformedness_0__LDIR_isAcyclicAux_match__3_splitter___redArg(lean_object* x_1, lean_object* x_2, lean_object* x_3) {
+_start:
+{
+lean_object* x_4; uint8_t x_5; 
+x_4 = lean_unsigned_to_nat(0u);
+x_5 = lean_nat_dec_eq(x_1, x_4);
+if (x_5 == 1)
+{
+lean_object* x_6; lean_object* x_7; 
+lean_dec(x_3);
+x_6 = lean_box(0);
+x_7 = lean_apply_1(x_2, x_6);
+return x_7;
+}
+else
+{
+lean_object* x_8; lean_object* x_9; lean_object* x_10; 
+lean_dec(x_2);
+x_8 = lean_unsigned_to_nat(1u);
+x_9 = lean_nat_sub(x_1, x_8);
+x_10 = lean_apply_1(x_3, x_9);
+return x_10;
+}
+}
+}
+LEAN_EXPORT lean_object* lp_LDIRProofs___private_LDIRProofs_proof__ir__wellformedness_0__LDIR_isAcyclicAux_match__3_splitter___redArg___boxed(lean_object* x_1, lean_object* x_2, lean_object* x_3) {
+_start:
+{
+lean_object* x_4; 
+x_4 = lp_LDIRProofs___private_LDIRProofs_proof__ir__wellformedness_0__LDIR_isAcyclicAux_match__3_splitter___redArg(x_1, x_2, x_3);
+lean_dec(x_1);
+return x_4;
+}
+}
+LEAN_EXPORT lean_object* lp_LDIRProofs___private_LDIRProofs_proof__ir__wellformedness_0__LDIR_isAcyclicAux_match__3_splitter(lean_object* x_1, lean_object* x_2, lean_object* x_3, lean_object* x_4) {
+_start:
+{
+lean_object* x_5; uint8_t x_6; 
+x_5 = lean_unsigned_to_nat(0u);
+x_6 = lean_nat_dec_eq(x_2, x_5);
+if (x_6 == 1)
+{
+lean_object* x_7; lean_object* x_8; 
+lean_dec(x_4);
+x_7 = lean_box(0);
+x_8 = lean_apply_1(x_3, x_7);
+return x_8;
+}
+else
+{
+lean_object* x_9; lean_object* x_10; lean_object* x_11; 
+lean_dec(x_3);
+x_9 = lean_unsigned_to_nat(1u);
+x_10 = lean_nat_sub(x_2, x_9);
+x_11 = lean_apply_1(x_4, x_10);
+return x_11;
+}
+}
+}
+LEAN_EXPORT lean_object* lp_LDIRProofs___private_LDIRProofs_proof__ir__wellformedness_0__LDIR_isAcyclicAux_match__3_splitter___boxed(lean_object* x_1, lean_object* x_2, lean_object* x_3, lean_object* x_4) {
+_start:
+{
+lean_object* x_5; 
+x_5 = lp_LDIRProofs___private_LDIRProofs_proof__ir__wellformedness_0__LDIR_isAcyclicAux_match__3_splitter(x_1, x_2, x_3, x_4);
+lean_dec(x_2);
+return x_5;
+}
+}
+LEAN_EXPORT lean_object* lp_LDIRProofs___private_LDIRProofs_proof__ir__wellformedness_0__LDIR_isAcyclicAux_match__1_splitter___redArg(lean_object* x_1, lean_object* x_2, lean_object* x_3) {
+_start:
+{
+if (lean_obj_tag(x_1) == 0)
+{
+lean_object* x_4; lean_object* x_5; 
+lean_dec(x_3);
+x_4 = lean_box(0);
+x_5 = lean_apply_1(x_2, x_4);
+return x_5;
+}
+else
+{
+lean_object* x_6; lean_object* x_7; 
+lean_dec(x_2);
+x_6 = lean_ctor_get(x_1, 0);
+lean_inc(x_6);
+lean_dec_ref(x_1);
+x_7 = lean_apply_1(x_3, x_6);
+return x_7;
+}
+}
+}
+LEAN_EXPORT lean_object* lp_LDIRProofs___private_LDIRProofs_proof__ir__wellformedness_0__LDIR_isAcyclicAux_match__1_splitter(lean_object* x_1, lean_object* x_2, lean_object* x_3, lean_object* x_4) {
+_start:
+{
+if (lean_obj_tag(x_2) == 0)
+{
+lean_object* x_5; lean_object* x_6; 
+lean_dec(x_4);
+x_5 = lean_box(0);
+x_6 = lean_apply_1(x_3, x_5);
+return x_6;
+}
+else
+{
+lean_object* x_7; lean_object* x_8; 
+lean_dec(x_3);
+x_7 = lean_ctor_get(x_2, 0);
+lean_inc(x_7);
+lean_dec_ref(x_2);
+x_8 = lean_apply_1(x_4, x_7);
+return x_8;
+}
+}
+}
+LEAN_EXPORT lean_object* lp_LDIRProofs___private_LDIRProofs_proof__ir__wellformedness_0__LDIR_payloadValid_match__1_splitter___redArg(lean_object* x_1, lean_object* x_2, lean_object* x_3) {
+_start:
+{
+if (lean_obj_tag(x_1) == 2)
+{
+lean_object* x_4; lean_object* x_5; 
+lean_dec(x_3);
+x_4 = lean_box(0);
+x_5 = lean_apply_1(x_2, x_4);
+return x_5;
+}
+else
+{
+lean_object* x_6; 
+lean_dec(x_2);
+x_6 = lean_apply_2(x_3, x_1, lean_box(0));
+return x_6;
+}
+}
+}
+LEAN_EXPORT lean_object* lp_LDIRProofs___private_LDIRProofs_proof__ir__wellformedness_0__LDIR_payloadValid_match__1_splitter(lean_object* x_1, lean_object* x_2, lean_object* x_3, lean_object* x_4) {
+_start:
+{
+if (lean_obj_tag(x_2) == 2)
+{
+lean_object* x_5; lean_object* x_6; 
+lean_dec(x_4);
+x_5 = lean_box(0);
+x_6 = lean_apply_1(x_3, x_5);
+return x_6;
+}
+else
+{
+lean_object* x_7; 
+lean_dec(x_3);
+x_7 = lean_apply_2(x_4, x_2, lean_box(0));
+return x_7;
+}
+}
+}
 lean_object* initialize_Init(uint8_t builtin);
 lean_object* initialize_Init(uint8_t builtin);
 static bool _G_initialized = false;
@@ -3487,6 +5347,10 @@ if (lean_io_result_is_error(res)) return res;
 lean_dec_ref(res);
 lp_LDIRProofs_LDIR_rootSentinel = _init_lp_LDIRProofs_LDIR_rootSentinel();
 lean_mark_persistent(lp_LDIRProofs_LDIR_rootSentinel);
+lp_LDIRProofs_LDIR_GIR__COMMAND__ARGS = _init_lp_LDIRProofs_LDIR_GIR__COMMAND__ARGS();
+lean_mark_persistent(lp_LDIRProofs_LDIR_GIR__COMMAND__ARGS);
+lp_LDIRProofs_LDIR_instInhabitedGIRCommand = _init_lp_LDIRProofs_LDIR_instInhabitedGIRCommand();
+lean_mark_persistent(lp_LDIRProofs_LDIR_instInhabitedGIRCommand);
 return lean_io_result_mk_ok(lean_box(0));
 }
 #ifdef __cplusplus
